KeyManagement/AdversarySafety.v
@@ -32,18 +32,79 @@ Module Automation.
 
   Import RealWorld.
 
+  Ltac solve_maps1 :=
+    match goal with
+    | [ |- context [ _ $+ (?k1,_) $? ?k2 ] ] =>
+      progress clean_map_lookups
+      || destruct (k1 ==n k2); subst; clean_map_lookups
+    | [ |- context [ ?m $? ?k ]] =>
+      progress context_map_rewrites
+      || cases (m $? k)
+    end.
+
+  Ltac process_keys_messages1 :=
+    match goal with
+    | [ H : msg_honestly_signed _ _ ?msg = _ |- _ ] => unfold msg_honestly_signed in H
+    | [ |- context [ msg_honestly_signed _ _ ?msg ] ] => unfold msg_honestly_signed; destruct msg; try discriminate; simpl in *
+    | [ |- let (_,_) := ?x in _] => destruct x
+    | [ H : context [ honest_keyb _ _ = _ ] |- _ ] => unfold honest_keyb in H
+    | [ |- context [ honest_keyb _ _ ] ] => unfold honest_keyb
+    | [ H : honest_key _ _ |- _ ] => invert H
+    | [ |- honest_key _ _ ] => constructor
+    | [ H : (if ?b then _ else _) = _ |- _ ] => is_var b; destruct b
+    | [ H : (match ?honk $? ?k with _ => _ end) = _ |- _ ] => cases (honk $? k)
+    | [ |- context [ if ?b then _ else _ ] ] => is_var b; destruct b
+    | [ |- context [ match ?c with _ => _ end ] ] =>
+      match type of c with
+      | cipher => destruct c
+      end
+    end.
+
+  Ltac process_keys_messages :=
+    repeat process_keys_messages1;
+    clean_context;
+    repeat solve_maps1;
+    try discriminate; try contradiction; context_map_rewrites.
+  
   Lemma message_honestly_signed_msg_signing_key_honest :
-    forall {t} (msg : crypto t) honestk,
-      msg_honestly_signed honestk msg = true
+    forall {t} (msg : crypto t) honestk cs,
+      msg_honestly_signed honestk cs msg  = true
       -> exists k,
-        msg_signing_key msg = Some k
+        msg_signing_key cs msg = Some k
         /\ honest_key honestk k.
   Proof.
     intros.
     unfold msg_honestly_signed in *; destruct msg; try discriminate;
-      rewrite <- honest_key_honest_keyb in *;
-      eexists; simpl; eauto.
+      repeat
+        match goal with
+        | [ H : (match ?m with _ => _ end) = _ |- _ ] => cases m; try discriminate; simpl in *
+        | [ H : Some _ = Some _ |- _ ] => invert H
+        | [ H : honest_keyb _ _ = true |- _] => rewrite <- honest_key_honest_keyb in H
+        end; eauto.
   Qed.
+
+  Lemma msg_honestly_signed_has_signing_key_cipher_id :
+    forall {t} (msg : crypto t) honestk cs,
+      msg_honestly_signed honestk cs msg = true
+      -> (exists k, msg_signing_key cs msg = Some k)
+        /\ (exists cid, msg_cipher_id msg = Some cid).
+  Proof.
+    unfold msg_honestly_signed, msg_signing_key, msg_cipher_id; intros.
+    destruct msg; try discriminate; repeat process_keys_messages; eauto.
+  Qed.
+
+  Lemma msg_honestly_signed_signing_key_honest :
+    forall {t} (msg : crypto t) honestk cs k,
+      msg_honestly_signed honestk cs msg = true
+      -> msg_signing_key cs msg = Some k
+      -> honest_key honestk k.
+  Proof.
+    unfold msg_honestly_signed, msg_signing_key; intros.
+    destruct msg; try discriminate; repeat process_keys_messages. constructor;
+      clean_context; eauto.
+  Qed.
+
+  Hint Resolve msg_honestly_signed_signing_key_honest.
 
   Ltac user_queue_lkup TAG :=
     match goal with
@@ -81,10 +142,10 @@ Module Automation.
   Ltac specialize_msg_queue_ok :=
     repeat
       match goal with
-      | [ H : (forall k, msg_signing_key ?msg = Some k -> _) |- _] =>
+      | [ H : (forall k, msg_signing_key _ ?msg = Some k -> _) |- _] =>
         match goal with
-        | [ MSK : msg_signing_key msg = Some _ |- _ ] => specialize (H _ MSK); split_ands
-        | [ MHS : msg_honestly_signed ?honk msg = true |- _ ] =>
+        | [ MSK : msg_signing_key _ msg = Some _ |- _ ] => specialize (H _ MSK); split_ands
+        | [ MHS : msg_honestly_signed ?honk _ msg = true |- _ ] =>
           apply message_honestly_signed_msg_signing_key_honest in MHS; split_ex; split_ands
         (* | _ => assert (msg_honestly_signed honk msg = true) as MHS by eauto *)
         end
@@ -92,23 +153,58 @@ Module Automation.
       end.
 
   Ltac specialize_msg_ok :=
-    repeat
+    repeat 
       match goal with
-      | [ H : (forall k, msg_signing_key _ = Some k -> _), MSK : msg_signing_key _ = Some _ |- _ ] => specialize (H _ MSK); split_ands
-      | [ H : (forall k, msg_signing_key _ = Some k -> _),
-          MPS : msg_pattern_safe ?honk _,
-          MAP :  msg_accepted_by_pattern _ ?msg |- _ ] =>
-        assert (msg_honestly_signed honk msg = true) as HON_SIGN by eauto;
-        generalize (message_honestly_signed_msg_signing_key_honest _ _ HON_SIGN); intros; split_ex; split_ands
-      (* eapply message_honestly_signed_msg_signing_key_honest in HON_SIGN; split_ex; split_ands *)
+      (* | [ H : (?arg -> _) , ARG : ?arg |- _ ] => specialize (H ARG) *)
+      | [ H : (forall k cid, msg_signing_key ?cs ?msg = Some k
+                        -> msg_cipher_id ?msg = Some cid
+                        -> _)
+      , MSK : msg_signing_key ?cs ?msg = Some _
+      , MCID : msg_cipher_id ?msg = Some _ |- _ ] => specialize (H _ _ MSK MCID); split_ands
+      | [ H : (forall k cid, msg_signing_key ?cs ?msg = Some k
+                        -> msg_cipher_id ?msg = Some cid
+                        -> _)
+      , MHS : msg_honestly_signed _ _ _ = true |- _ ] => 
+        generalize (msg_honestly_signed_has_signing_key_cipher_id _ _ _ MHS); intros; split_ands; split_ex
+      | [ MPS : msg_pattern_safe ?honk _
+        , MAP :  msg_accepted_by_pattern ?cs _ ?msg |- _ ] =>
+        assert_if_new (msg_honestly_signed honk cs msg = true) eauto
+      | [ H1 : msg_honestly_signed ?honk _ ?msg = true, H2 : msg_signing_key _ ?msg = Some ?k |- _ ] =>
+        assert_if_new (honest_key honk k) eauto
+      (* | [ OK : msgCipherOk ?cs ?msg, H : (msgCipherOk ?cs ?msg -> _) |- _] => specialize (H OK); split_ands *)
+      | [ H : (forall k kp, findKeysCrypto ?cs ?msg $? k = Some kp -> _), ARG : findKeysCrypto ?cs ?msg $? _ = Some _ |- _ ] =>
+          specialize (H _ _ ARG)
       | [ HK : honest_key ?honk ?k, H : (honest_key ?honk ?k -> _) |- _] => specialize (H HK); split_ands
+      | [ HL : ?honk $? ?k = Some true, H : (honest_key ?honk ?k -> _) |- _] =>
+        assert (honest_key honk k) as HK by (constructor; auto); specialize (H HK); split_ands
+      | [ PK : ?pubk $? _ = Some _, H : (forall k p, ?pubk $? k = Some p -> _) |- _ ] => specialize (H _ _ PK); split_ands
+      | [ MC : msg_cipher_id ?c = Some _, H : (forall cid, msg_cipher_id ?c = Some cid -> _) |- _ ] =>
+        specialize (H _ MC); split_ands
       end.
-
+    (* repeat *)
+    (*   match goal with *)
+    (*   | [ H : (forall k, msg_signing_key _ = Some k -> _), MSK : msg_signing_key _ = Some _ |- _ ] => specialize (H _ MSK); split_ands *)
+    (*   | [ H : (forall k, msg_signing_key _ = Some k -> _), *)
+    (*       MPS : msg_pattern_safe ?honk _, *)
+    (*       MAP :  msg_accepted_by_pattern _ ?msg |- _ ] => *)
+    (*     assert (msg_honestly_signed honk msg = true) as HON_SIGN by eauto; *)
+    (*     generalize (message_honestly_signed_msg_signing_key_honest _ _ HON_SIGN); intros; split_ex; split_ands *)
+    (*   (* eapply message_honestly_signed_msg_signing_key_honest in HON_SIGN; split_ex; split_ands *) *)
+    (*   | [ HK : honest_key ?honk ?k, H : (honest_key ?honk ?k -> _) |- _] => specialize (H HK); split_ands *)
+    (*   | [ HL : ?honk $? ?k = Some true, H : (honest_key ?honk ?k -> _) |- _] => *)
+    (*     assert (honest_key honk k) as HK by (constructor; auto); specialize (H HK); split_ands *)
+    (*   | [ PK : ?pubk $? _ = Some _, H : (forall k p, ?pubk $? k = Some p -> _) |- _ ] => specialize (H _ _ PK); split_ands *)
+    (*   | [ MC : msg_cipher_id ?c = Some _, H : (forall cid, msg_cipher_id ?c = Some cid -> _) |- _ ] => *)
+    (*     specialize (H _ MC); split_ands *)
+    (*   end. *)
+                   
   Ltac msg_queue_prop :=
     match goal with
-    | [ OK : message_queues_ok _ ?us _ |- _ ] =>
+    | [ OK : message_queues_ok ?cs ?us ?gks |- _ ] =>
       match goal with
-      | [ H : us $? _ = Some _ |- _ ] => generalize (Forall_natmap_in_prop _ OK H); simpl; intros
+      | [ H : us $? _ = Some ?u |- _ ] =>
+        prop_not_unifies (message_queue_ok (findUserKeys us) cs (msg_heap u) gks);
+        generalize (Forall_natmap_in_prop _ OK H); simpl; intros
       | _ => let USR := fresh "USR"
             in user_queue_lkup USR;
                do 3 (destruct USR as [?x USR]);
@@ -129,7 +225,7 @@ Module Automation.
         (* end *)
       (* | [ H1: msg_honestly_signed _ _ = true -> _, H2: msg_honestly_signed _ _ = true |- _ ] => *)
       (*   specialize (H1 H2); split_ands *)
-      | [ MHS : msg_honestly_signed _ ?msg = _ , MTCH : match ?msg with _ => _ end |- _ ] =>
+      | [ MHS : msg_honestly_signed _ _ ?msg = _ , MTCH : match ?msg with _ => _ end |- _ ] =>
         unfold msg_honestly_signed in MHS; destruct msg; try discriminate; rewrite MHS in *;
         split_ands; simpl in *
       end.
@@ -155,9 +251,11 @@ Module Automation.
 
   Ltac user_cipher_queues_prop :=
     match goal with
-    | [ OK : user_cipher_queues_ok _ _ ?us |- _ ] => 
+    | [ OK : user_cipher_queues_ok ?cs ?honk ?us |- _ ] => 
       match goal with
-      | [ H : us $? _ = Some _ |- _ ] => generalize (Forall_natmap_in_prop _ OK H); simpl; intros
+      | [ H : us $? _ = Some ?u |- _ ] =>
+        prop_not_unifies (user_cipher_queue_ok cs honk (c_heap u));
+        generalize (Forall_natmap_in_prop _ OK H); simpl; intros
       | _ => let USR := fresh "USR"
             in user_cipher_queue_lkup USR;
             do 3 (destruct USR as [?x USR]);
@@ -176,9 +274,11 @@ Module Automation.
 
   Ltac permission_heaps_prop :=
     match goal with
-    | [ OK : Forall_natmap (fun _ => permission_heap_good _ _) ?us |- _ ] => 
+    | [ OK : Forall_natmap (fun _ => permission_heap_good ?gks _) ?us |- _ ] => 
       match goal with
-      | [ H : us $? _ = Some _ |- _ ] => generalize (Forall_natmap_in_prop _ OK H); simpl; intros
+      | [ H : us $? _ = Some ?u |- _ ] =>
+        prop_not_unifies (permission_heap_good gks (key_heap u));
+        generalize (Forall_natmap_in_prop _ OK H); simpl; intros
       | _ => let USR := fresh "USR"
             in user_keys_lkup USR;
                do 3 (destruct USR as [?x USR]);
@@ -186,6 +286,17 @@ Module Automation.
       end
     end.
   
+  Ltac keys_and_permissions_prop :=
+    match goal with
+    | [ H : keys_and_permissions_good ?gks ?usrs ?adv |- _ ] =>
+      assert (keys_and_permissions_good gks usrs adv) as KPG by assumption; unfold keys_and_permissions_good in KPG; split_ands;
+      permission_heaps_prop
+      (* match goal with *)
+      (* | [H1 : ?usrs $? _ = Some _, H2 : Forall_natmap (fun u => permission_heap_good _ _) ?usrs |- _ ] => *)
+      (*   generalize (Forall_natmap_in_prop _ H2 H1); simpl; intros *)
+      (* end *)
+    end.
+
   Ltac encrypted_ciphers_prop :=
     match goal with
     | [ H  : encrypted_ciphers_ok _ (?cs $+ (?cid,?c)) _ |- _ ] => generalize (Forall_natmap_in_prop_add H); intros
@@ -195,16 +306,6 @@ Module Automation.
            | [ H : encrypted_cipher_ok _ _ _ _ |- _ ] => invert H
            | [ H : honest_keyb _ _ = true |- _] => apply honest_keyb_true_findKeys in H
            end; try contradiction.
-
-  Ltac keys_and_permissions_prop :=
-    match goal with
-    | [ H : keys_and_permissions_good ?gks ?usrs ?adv |- _ ] =>
-      assert (keys_and_permissions_good gks usrs adv) as KPG by assumption; unfold keys_and_permissions_good in KPG; split_ands;
-      match goal with
-      | [H1 : ?usrs $? _ = Some _, H2 : Forall_natmap (fun u => permission_heap_good _ _) ?usrs |- _ ] =>
-        generalize (Forall_natmap_in_prop _ H2 H1); simpl; intros
-      end
-    end.
 
   Ltac refine_signed_messages :=
     repeat
@@ -221,31 +322,6 @@ Module Automation.
       | [ COND : honest_keyb ?honk ?kid = _
         , H : if honest_keyb ?honk ?kid then _ else _ |- _ ] => rewrite COND in H
       end; split_ands.
-
-  Ltac solve_maps1 :=
-    match goal with
-    | [ |- context [ _ $+ (?k1,_) $? ?k2 ] ] =>
-      progress clean_map_lookups
-      || destruct (k1 ==n k2); subst; clean_map_lookups
-    | [ |- context [ ?m $? ?k ]] =>
-      progress context_map_rewrites
-      || cases (m $? k)
-    end.
-
-  Ltac process_keys_messages1 :=
-    match goal with
-    | [ H : msg_honestly_signed _ ?msg = _ |- _ ] => unfold msg_honestly_signed in H
-    | [ |- context [ msg_honestly_signed _ ?msg ] ] => unfold msg_honestly_signed; destruct msg; try discriminate
-    | [ |- let (_,_) := ?x in _] => destruct x
-    | [ H : honest_keyb _ _ = _ |- _ ] => unfold honest_keyb in H
-    | [ |- context [ honest_keyb _ _ ] ] => unfold honest_keyb
-    | [ |- context [ if ?b then _ else _ ] ] => is_var b; destruct b
-    end.
-
-  Ltac process_keys_messages :=
-    repeat process_keys_messages1;
-    repeat solve_maps1;
-    try discriminate; try contradiction; context_map_rewrites.
 
   Hint Resolve
        clean_honest_key_permissions_distributes
@@ -310,19 +386,19 @@ Section UniverseLemmas.
     |}.
 
   Lemma adv_no_honest_keys_after_honestk_no_private_key_msg :
-    forall {t} (msg : crypto t) honestk advk,
+    forall {t} (msg : crypto t) honestk cs advk,
       adv_no_honest_keys honestk advk
-      -> (forall (k_id : NatMap.key) (kp : bool), findKeysCrypto msg $? k_id = Some kp -> kp = false)
-      -> adv_no_honest_keys (honestk $k++ findKeysCrypto msg) advk.
+      -> (forall (k_id : NatMap.key) (kp : bool), findKeysCrypto cs msg $? k_id = Some kp -> kp = false)
+      -> adv_no_honest_keys (honestk $k++ findKeysCrypto cs msg) advk.
   Proof.
     unfold adv_no_honest_keys; intros; eauto;
       match goal with
       | [ kid : ?T, H : forall _ : ?T, _ \/ _ |- _ ] => specialize (H kid)
       end;
         split_ors; intuition idtac;
-        cases (findKeysCrypto msg $? k_id);
+        cases (findKeysCrypto cs msg $? k_id);
         try match goal with
-            | [ H1 : findKeysCrypto _ $? ?k_id = Some ?kp
+            | [ H1 : findKeysCrypto _ _ $? ?k_id = Some ?kp
               , H2 : forall k p, _ |- _ ] => specialize (H2 _ _ H1)
             end;
         subst; simplify_key_merges1; auto.
@@ -333,7 +409,7 @@ Section UniverseLemmas.
       msgCiphersSignedOk honestk cs msg
       -> msgCiphersSignedOk (honestk $k++ msgk) cs msg.
   Proof.
-    unfold msgCiphersSignedOk, msgCipherOk.
+    unfold msgCiphersSignedOk.
     induction 1; eauto.
     econstructor; intuition eauto;
       match goal with
@@ -346,12 +422,12 @@ Section UniverseLemmas.
       msgCiphersSignedOk honestk cs msg
       -> msgCiphersSignedOk (honestk $+ (k_id,true)) cs msg.
   Proof.
-    unfold msgCiphersSignedOk, msgCipherOk.
+    unfold msgCiphersSignedOk.
     induction 1; eauto.
     econstructor; eauto;
       match goal with
       | [ |- let (_,_) := ?x in _] => destruct x
-      end; intuition eauto; process_keys_messages; eauto.
+      end; intuition eauto; repeat process_keys_messages; eauto.
   Qed.
 
   Hint Resolve msgCiphersSigned_after_msg_keys msgCiphersSigned_new_private_key.
@@ -359,10 +435,10 @@ Section UniverseLemmas.
   (* Step keys and permissions good *)
 
   Lemma keys_and_permissions_good_user_new_pubk :
-    forall {A t} (usrs : honest_users A) gks (msg : crypto t) u_id u_d ks cmd qmsgs mycs adv_heap,
+    forall {A t} (usrs : honest_users A) gks (msg : message t) u_id u_d ks cmd qmsgs mycs adv_heap,
       keys_and_permissions_good gks usrs adv_heap
-      -> (forall (k : NatMap.key) (kp : bool), findKeysCrypto msg $? k = Some kp -> gks $? k <> None)
-      -> u_d = {| key_heap := ks $k++ findKeysCrypto msg
+      -> (forall (k : NatMap.key) (kp : bool), findKeysMessage msg $? k = Some kp -> gks $? k <> None)
+      -> u_d = {| key_heap := ks $k++ findKeysMessage msg
                ; msg_heap := qmsgs
                ; protocol := cmd
                ; c_heap := mycs |}
@@ -375,7 +451,7 @@ Section UniverseLemmas.
 
     permission_heaps_prop.
     unfold permission_heap_good; intros.
-    cases (ks $? k_id); cases (findKeysCrypto msg $? k_id); simplify_key_merges1; clean_map_lookups; eauto.
+    cases (ks $? k_id); cases (findKeysMessage msg $? k_id); simplify_key_merges1; clean_map_lookups; eauto.
     cases (gks $? k_id); eauto.
     exfalso; eauto.
   Qed.
@@ -427,7 +503,11 @@ Section UniverseLemmas.
       eauto;
       process_permission_heaps;
       permission_heaps_prop;
-      eauto.
+      specialize_msg_ok;
+      eauto;
+      clean_map_lookups.
+
+    cases (gks' $? k_id); try contradiction; eauto.
   Qed.
 
   Lemma permission_heap_good_addnl_key :
@@ -519,11 +599,12 @@ Section UniverseLemmas.
       try discriminate; eauto 2; clean_context.
 
     - user_cipher_queues_prop;
-        encrypted_ciphers_prop; eapply keys_and_permissions_good_user_new_pubk; eauto; intros; eauto.
+        encrypted_ciphers_prop.
+      eapply keys_and_permissions_good_user_new_pubk; eauto; intros; eauto.
       specialize (H16 _ _ H4); split_ands; subst.
       keys_and_permissions_prop; eauto.
       assert (permission_heap_good gks' (findUserKeys usrs')) by eauto.
-      specialize (H18 _ _ H6); split_ex; intuition contra_map_lookup.
+      specialize (H17 _ _ H6); split_ex; intuition contra_map_lookup.
 
     - unfold keys_and_permissions_good in *; intuition eauto.
       + destruct (k_id ==n k_id0); subst; clean_map_lookups; eauto.
@@ -585,8 +666,8 @@ Section UniverseLemmas.
       unfold permission_heap_good in *; intros.
       cases (key_heap adv' $? k_id); eauto.
       invert H16; split_ands.
-      cases (findKeysCrypto msg $? k_id); simplify_key_merges1; try discriminate.
-      specialize (H3 _ _ Heq0); split_ands; subst.
+      cases (findKeysCrypto cs' msg $? k_id); simplify_key_merges1; try discriminate.
+      specialize (H4 _ _ Heq0); split_ands; subst.
       cases (gks' $? k_id); try contradiction; eauto.
     - destruct rec_u; simpl in *.
       eapply keys_and_permissions_good_readd_user_same_perms; eauto.
@@ -596,7 +677,7 @@ Section UniverseLemmas.
       encrypted_ciphers_prop; clean_map_lookups; eauto.
       + specialize (H17 _ _ H5); split_ex; intuition eauto.
       + assert (permission_heap_good gks' (findUserKeys usrs')) by eauto.
-        specialize (H18 _ _ H5); split_ands; subst.
+        specialize (H21 _ _ H5); split_ands; subst.
         specialize (H9 _ _ H10); eauto.
 
     - unfold keys_and_permissions_good in *; intuition eauto.
@@ -623,11 +704,11 @@ Section UniverseLemmas.
   Hint Resolve permission_heap_good_clean_keys.
 
   Lemma keys_and_permissions_good_clean_keys :
-    forall {A} (usrs : honest_users A) adv_heap gks,
+    forall {A} (usrs : honest_users A) adv_heap cs gks,
       keys_and_permissions_good gks usrs adv_heap
       -> keys_and_permissions_good
           (clean_keys (findUserKeys usrs) gks)
-          (clean_users (findUserKeys usrs) usrs)
+          (clean_users (findUserKeys usrs) cs usrs)
           (clean_key_permissions (findUserKeys usrs) adv_heap).
   Proof.
     unfold keys_and_permissions_good; intros; split_ands.
@@ -638,7 +719,7 @@ Section UniverseLemmas.
         match goal with
         | [ H : clean_keys _ _ $? _ = Some _ |- _ ] => eapply clean_keys_inv in H; split_ands
         | [ H : clean_keys _ _ $? _ = None |- _ ] => eapply clean_keys_inv' in H; split_ands
-        | [ H : clean_users _ _ $? _ = Some _ |- _ ] => eapply clean_users_cleans_user_inv in H; split_ex; split_ands
+        | [ H : clean_users _ _ _ $? _ = Some _ |- _ ] => eapply clean_users_cleans_user_inv in H; split_ex; split_ands
         end.
     
     - inv_cleans; eauto.
@@ -776,13 +857,21 @@ Section UniverseLemmas.
   Lemma msgCiphersSignedOk_user_cipher_queue_ok_findCiphers :
     forall {t} (msg : crypto t) honestk cs,
       msgCiphersSignedOk honestk cs msg
-      -> user_cipher_queue_ok cs (honestk $k++ findKeysCrypto msg) (findCiphers msg).
+      -> user_cipher_queue_ok cs (honestk $k++ findKeysCrypto cs msg) (findCiphers msg).
   Proof.
     induction msg;
       intros;
       unfold user_cipher_queue_ok in *;
       repeat
         match goal with
+        | [ H : msg_honestly_signed _ _ (SignedCiphertext ?cid) = true |- _ ] =>
+          unfold msg_honestly_signed, msg_signing_key in H;
+            cases (cs $? cid); try discriminate;
+              destruct c; try discriminate; simpl in H
+        (* | [ H : msg_honestly_signed _ _ (Signature _ ?cid) = true |- _ ] => *)
+        (*   unfold msg_honestly_signed, msg_signing_key in H; *)
+        (*     cases (cs $? cid); try discriminate; *)
+        (*       destruct c; try discriminate *)
         | [ H : msgCiphersSignedOk _ _ _ |- _ ] => invert H; simpl in *; split_ands; split_ex
         | [ H : honest_keyb _ _ = true |- _ ] => apply honest_keyb_true_findKeys in H
         | [ |- Forall _ _ ] => econstructor
@@ -800,7 +889,7 @@ Section UniverseLemmas.
     forall {t} (msg : crypto t) cs honestk mycs,
       user_cipher_queue_ok cs honestk mycs
       -> msgCiphersSignedOk honestk cs msg
-      -> user_cipher_queue_ok cs (honestk $k++ findKeysCrypto msg) (findCiphers msg ++ mycs).
+      -> user_cipher_queue_ok cs (honestk $k++ findKeysCrypto cs msg) (findCiphers msg ++ mycs).
   Proof.
     induction 1; unfold msgCiphersSignedOk; intros.
     - rewrite app_nil_r; eauto.
@@ -820,7 +909,7 @@ Section UniverseLemmas.
       user_cipher_queues_ok cs (findUserKeys usrs) usrs
       -> usrs $? u_id = Some {| key_heap := ks; protocol := cmd; msg_heap := qmsgs; c_heap := mycs |}
       -> msgCiphersSignedOk (findUserKeys usrs) cs msg
-      -> usrs' = usrs $+ (u_id, {| key_heap := ks $k++ findKeysCrypto msg; protocol := cmd'; msg_heap := qmsgs'; c_heap := findCiphers msg ++ mycs |})
+      -> usrs' = usrs $+ (u_id, {| key_heap := ks $k++ findKeysCrypto cs msg; protocol := cmd'; msg_heap := qmsgs'; c_heap := findCiphers msg ++ mycs |})
       -> honestk = findUserKeys usrs'
       -> user_cipher_queues_ok cs honestk usrs'.
   Proof.
@@ -944,10 +1033,6 @@ Section UniverseLemmas.
          simpl; unfold honest_keyb; context_map_rewrites; eauto.
       +  eapply user_cipher_queues_ok_addnl_global_cipher; eauto.
 
-    - encrypted_ciphers_prop; clean_map_lookups.
-      eapply user_cipher_queues_ok_add_user; eauto.
-      autorewrite with find_user_keys; trivial.
-      
     - econstructor; simpl; eauto.
       + econstructor; clean_map_lookups; eauto.
         eexists; intuition eauto.
@@ -980,9 +1065,9 @@ Section UniverseLemmas.
   (* Message queues ok step *)
 
   Lemma message_no_adv_private_new_keys :
-    forall {t} (msg : crypto t) honestk pubk,
-      message_no_adv_private honestk msg
-      -> message_no_adv_private (honestk $k++ pubk) msg.
+    forall {t} (msg : crypto t) honestk cs pubk,
+      message_no_adv_private honestk cs msg
+      -> message_no_adv_private (honestk $k++ pubk) cs msg.
   Proof.
     unfold message_no_adv_private; intros.
     specialize (H _ _ H0).
@@ -990,9 +1075,9 @@ Section UniverseLemmas.
   Qed.
 
   Lemma message_no_adv_private_new_honestk :
-    forall {t} (msg : crypto t) honestk k_id,
-      message_no_adv_private honestk msg
-      -> message_no_adv_private (honestk $+ (k_id,true)) msg.
+    forall {t} (msg : crypto t) honestk cs k_id,
+      message_no_adv_private honestk cs msg
+      -> message_no_adv_private (honestk $+ (k_id,true)) cs msg.
   Proof.
     unfold message_no_adv_private; intros.
     specialize (H _ _ H0).
@@ -1010,15 +1095,34 @@ Section UniverseLemmas.
     unfold message_queue_ok; induction 1; eauto; intros;
       econstructor; eauto.
 
-    destruct x; simpl in *; split_ands; split_ands; split; eauto; intros.
-    specialize (H2 _ H3); split_ands; split; intros; eauto.
-    invert H5; apply merge_perms_split in H6; split_ors.
-    - assert (honest_key honestk k) by (constructor; auto).
-      specialize (H4 H6); split_ands; eauto.
-    - specialize (H1 _ _ H5); split_ands; discriminate.
+    destruct x; simpl in *; intuition eauto;
+      specialize_msg_ok; eauto;
+        repeat
+          match goal with
+          | [ H : honest_key (_ $k++ _) _ |- _ ] => invert H
+          | [ H : _ $k++ _ $? _ = Some true |- _ ] => apply merge_perms_split in H; split_ors
+          end;
+        specialize_msg_ok; eauto.
   Qed.
 
   Hint Resolve message_queue_ok_adding_public_keys.
+
+  Lemma message_queues_ok_user_adding_public_keys :
+    forall {A} (usrs usrs' : honest_users A) cs gks u_id pubk ks cmd cmd' msg msgs mycs mycs',
+      message_queues_ok cs usrs gks
+      -> (forall k p, pubk $? k = Some p -> (findUserKeys usrs) $? k = Some true /\ p = false)
+      -> usrs $? u_id = Some {| key_heap := ks; protocol := cmd; msg_heap := msg::msgs; c_heap := mycs |}
+      -> usrs' = usrs $+ (u_id, {| key_heap := ks $k++ pubk; protocol := cmd'; msg_heap := msgs; c_heap := mycs' |})
+      -> message_queues_ok cs usrs' gks.
+  Proof.
+    intros; subst.
+    unfold message_queues_ok in *; rewrite Forall_natmap_forall in *; intros.
+    destruct (u_id ==n k); subst; clean_map_lookups; autorewrite with find_user_keys; eauto; simpl.
+    eapply message_queue_ok_adding_public_keys; eauto.
+    specialize (H _ _ H1); invert H; eauto.
+  Qed.
+
+  Hint Resolve message_queues_ok_user_adding_public_keys.
 
   Lemma message_queues_ok_readd_user_same_queue :
     forall {A} (usrs : honest_users A) cs u_id ks cmd cmd' qmsgs mycs mycs' gks,
@@ -1046,7 +1150,28 @@ Section UniverseLemmas.
 
   Hint Resolve
        message_queues_ok_readd_user_popped_queue
-       msgCiphersSignedOk_addnl_cipher.
+       (* msgCipherOk_addnl_cipher *)
+       msgCiphersSignedOk_addnl_cipher
+       msgCiphersSignedOk_new_honest_key'.
+
+  (* Lemma msgCipherOk_split : *)
+  (*   forall {t} (msg : crypto t) cs cid1 cid2 c, *)
+  (*     ~ In cid1 cs *)
+  (*     -> msg_cipher_id msg = Some cid2 *)
+  (*     -> msgCipherOk (cs $+ (cid1,c)) msg *)
+  (*     -> (cid1 <> cid2 /\ msgCipherOk cs msg) *)
+  (*     \/ (cid1 = cid2 /\ match msg with *)
+  (*                      | Content _ => False *)
+  (*                      | SignedCiphertext k__sign k__enc msg_id => *)
+  (*                        exists (t1 : message.type) (m' : crypto t1), c = SigEncCipher k__sign k__enc m' *)
+  (*                      | Signature m' k sig => c = SigCipher k m' *)
+  (*                      end). *)
+  (* Proof. *)
+  (*   intros. *)
+  (*   destruct (cid1 ==n cid2); subst; *)
+  (*     unfold msgCipherOk, msg_cipher_id in *; destruct msg; *)
+  (*       split_ex; clean_map_lookups; eauto. *)
+  (* Qed. *)
 
   Lemma message_queue_ok_addnl_cipher :
     forall msgs cs honestk c_id c gks,
@@ -1054,11 +1179,21 @@ Section UniverseLemmas.
       -> ~ In c_id cs
       -> message_queue_ok honestk (cs $+ (c_id, c)) msgs gks.
   Proof.
-    induction 1; unfold message_queue_ok in *; intros; econstructor; eauto.
+    unfold message_queue_ok; induction 1; eauto; intros;
+      econstructor; eauto.
+
+    destruct x; simpl in *; split_ands.
+    split; intros; eauto; specialize_msg_ok.
+    admit.
     
-    destruct x; simpl in *; intros; split_ands; split; eauto; intros.
-    specialize (H2 _ H3); intuition eauto.
-  Qed.
+
+    (* assert (msg_signing_key cs c0 = Some k). *)
+    (* unfold msg_signing_key in *; destruct c0; try discriminate; eauto. *)
+    (* destruct (c_id ==n msg_id); subst; clean_map_lookups; eauto. *)
+
+    (* intuition eauto. *)
+    (* destruct (c_id ==n cid); subst; clean_map_lookups; eauto. *)
+  Admitted.
 
   Hint Resolve message_queue_ok_addnl_cipher.
 
@@ -1068,12 +1203,7 @@ Section UniverseLemmas.
       -> ~ In c_id cs
       -> message_queues_ok (cs $+ (c_id,c)) usrs gks.
   Proof.
-    unfold message_queues_ok; intros; rewrite Forall_natmap_forall in *; intros.
-    specialize (H _ _ H1).
-    unfold message_queue_ok in *; rewrite Forall_forall in *; intros.
-    specialize (H _ H2); destruct x; split_ands.
-    split; eauto; intros.
-    specialize (H3 _ H4); intuition eauto.
+    unfold message_queues_ok in *; intros; rewrite Forall_natmap_forall in *; intros; eauto.
   Qed.
 
   Hint Resolve message_queues_ok_addnl_cipher.
@@ -1094,26 +1224,42 @@ Section UniverseLemmas.
 
   Hint Resolve new_global_key_not_in_heaps.
 
+  Lemma msg_signing_key_cipher_id_in_ciphers :
+    forall {t} (c : crypto t) cs k_id c_id,
+      msg_signing_key cs c = Some k_id
+      -> msg_cipher_id c = Some c_id
+      -> exists c, cs $? c_id = Some c
+             /\ (exists {t} (m : message t),
+                   c = SigCipher k_id m
+                 \/ exists k__enc, c = SigEncCipher k_id k__enc m).
+  Proof.
+    intros.
+    unfold msg_signing_key, msg_cipher_id in *.
+    destruct c; try discriminate; invert H0;
+      cases (cs $? c_id); try discriminate.
+
+    destruct c; try discriminate; clean_context;
+      eexists; split; eauto.
+  Qed.
+
   Lemma message_queue_ok_addnl_honest_key :
     forall msgs cs honestk k_id gks usage kt,
       message_queue_ok honestk cs msgs gks
-      -> ~ In k_id gks
-      -> ~ In k_id honestk
-      -> permission_heap_good gks honestk
+      -> gks $? k_id = None
+      -> honestk $? k_id = None
+      -> encrypted_ciphers_ok honestk cs gks
       -> message_queue_ok (honestk $+ (k_id,true)) cs msgs (gks $+ (k_id, {| keyId := k_id; keyUsage := usage; keyType := kt |} )).
   Proof.
     induction 1; intros; econstructor; unfold message_queue_ok in *; eauto.
 
     destruct x; simpl in *; intros.
     assert (honestk $? k_id = None) by eauto.
-    split_ands.
-    split; intros.
-    + destruct (k_id ==n k); subst; clean_map_lookups; eauto.
-    + specialize (H5 _ H6).
-      destruct (k_id ==n k); subst; clean_map_lookups; intuition eauto;
-        invert H5;
-        clean_map_lookups;
-        assert (honest_key honestk k) as HK by (constructor; auto); specialize (H8 HK); split_ands; eauto.
+    split; intros; split_ands; specialize_msg_ok.
+    - unfold not; intros; destruct (k_id ==n k); subst; split_ands; clean_map_lookups; specialize_msg_ok; eauto.
+    - destruct (k_id ==n k); subst; clean_map_lookups; split_ands; try contradiction; eauto.
+      split; eauto.
+      split; eauto; intros.
+      invert H10; clean_map_lookups; specialize_msg_ok; eauto.
   Qed.
 
   Lemma message_queue_ok_addnl_adv_key :
@@ -1126,23 +1272,17 @@ Section UniverseLemmas.
     induction 1; intros; econstructor; eauto.
     - destruct x; simpl in *; intros.
       assert (honestk $? k_id = None) by eauto.
-      split_ands.
-      split; intros.
+      intuition eauto; specialize_msg_ok; eauto.
       + destruct (k_id ==n k); subst; clean_map_lookups; eauto.
-      + specialize (H4 _ H5).
-        destruct (k_id ==n k); subst; clean_map_lookups; intuition eauto;
-          invert H5;
-          clean_map_lookups;
-          assert (honest_key honestk k) as HK by (constructor; auto); specialize (H8 HK); split_ands; eauto.
+      + destruct (k_id ==n k); subst; clean_map_lookups; specialize_msg_ok; eauto.
     - eapply IHForall; eauto.
-
   Qed.
-
 
   Lemma message_queues_ok_addnl_honest_key :
     forall {A} (usrs : honest_users A) cs u_id k_id gks ks cmd cmd' qmsgs mycs usage kt,
       message_queues_ok cs usrs gks
       -> ~ In k_id gks
+      -> encrypted_ciphers_ok (findUserKeys usrs) cs gks
       -> permission_heap_good gks (findUserKeys usrs)
       -> usrs $? u_id = Some {| key_heap := ks; protocol := cmd; msg_heap := qmsgs; c_heap := mycs |}
       -> message_queues_ok cs
@@ -1187,14 +1327,95 @@ Section UniverseLemmas.
   Hint Resolve content_only_honest_public_keys_findkeys_no_priv.
 
   Lemma message_contains_only_honest_public_keys_findkeys_no_priv :
-    forall {t} (msg : crypto t) k honestk,
-      msg_contains_only_honest_public_keys honestk msg
-      -> findKeysCrypto msg $? k <> Some true.
+    forall {t} (msg : crypto t) k honestk cs,
+      msg_contains_only_honest_public_keys honestk cs msg
+      -> findKeysCrypto cs msg $? k <> Some true.
   Proof.
-    induction 1; simpl; intros; clean_map_lookups; eauto.
+    induction 1; simpl; intros; eauto;
+      context_map_rewrites; clean_map_lookups; eauto.
   Qed.
 
   Hint Resolve message_contains_only_honest_public_keys_findkeys_no_priv.
+
+  (* Lemma msg_contains_only_honest_public_keys_message_no_adv_private : *)
+  (*   forall {t} (msg : crypto t) honestk cs, *)
+  (*     msg_contains_only_honest_public_keys honestk cs msg *)
+  (*     -> msg_honestly_signed honestk cs msg = true *)
+  (*     -> msgCiphersSignedOk honestk cs msg *)
+  (*     -> message_no_adv_private honestk msg. *)
+  (* Proof. *)
+  (*   induction msg; intros; try discriminate; eauto. *)
+
+    
+  (*   induction 1; intros; *)
+  (*     try discriminate; eauto. *)
+
+  (*   unfold msgCiphersSignedOk in H1; simpl in H1; invert H1. *)
+  (*   unfold message_no_adv_private in *; intros. *)
+  (*   eapply IHmsg_contains_only_honest_public_keys; eauto. *)
+    
+  (*   rewrite Forall_forall in H5; eauto. *)
+
+
+    
+    
+    
+
+  (*   unfold message_no_adv_private in *; intros; simpl in *; eauto. *)
+  (*   unfold msg_honestly_signed in H0. *)
+    
+
+  (*     H20 : user_cipher_queues_ok cs' (findUserKeys usrs) usrs *)
+  (* H : msg_contains_only_honest_public_keys (findUserKeys usrs) cs' msg *)
+  (* H2 : msg_honestly_signed (findUserKeys usrs) cs' msg = true *)
+  (* H5 : msgCiphersSignedOk (findUserKeys usrs) cs' msg *)
+  (* cmdc, cmdc' : user_cmd A *)
+  (* H32 : usrs $? u_id = Some {| key_heap := ks'; protocol := cmdc; msg_heap := qmsgs'; c_heap := mycs' |} *)
+  (* H6 : message_queue_ok (findUserKeys usrs) cs' qmsgs' gks' *)
+  (* H10 : permission_heap_good gks' ks' *)
+  (* H11 : message_queue_ok (findUserKeys usrs) cs' (msg_heap rec_u) gks' *)
+  (* k : key_identifier *)
+  (* cid : cipher_id *)
+  (* H12 : msg_signing_key cs' msg = Some k *)
+  (* H13 : msg_cipher_id msg = Some cid *)
+  (* H14 : honest_key (findUserKeys usrs) k *)
+  (* H15 : user_cipher_queue_ok cs' (findUserKeys usrs) mycs' *)
+  (* H16 : user_cipher_queue_ok cs' (findUserKeys usrs) (c_heap rec_u) *)
+  (* ============================ *)
+  (* message_no_adv_private (findUserKeys usrs) msg *)
+
+  Lemma msg_cipher_id_in_mycs :
+    forall {t} (msg : crypto t) mycs c_id,
+      incl (findCiphers msg) mycs
+      -> msg_cipher_id msg = Some c_id
+      -> List.In c_id mycs.
+  Proof.
+    intros; destruct msg; simpl in *; try discriminate;
+      clean_context; eauto.
+  Qed.
+
+  Hint Resolve msg_cipher_id_in_mycs.
+    
+  Lemma honestly_signed_message_in_key_heap :
+    forall {t} (msg : crypto t) honestk cs gks k_id,
+      msg_honestly_signed honestk cs msg = true
+      (* -> incl (findCiphers msg) mycs *)
+      -> permission_heap_good gks honestk
+      (* -> encrypted_ciphers_ok honestk cs gks *)
+      (* -> user_cipher_queue_ok cs honestk mycs *)
+      -> msg_signing_key cs msg = Some k_id
+      (* -> msg_cipher_id msg = Some c_id *)
+      (* -> cs $? c_id <> None *)
+      -> gks $? k_id <> None.
+  Proof.
+    intros.
+    unfold msg_honestly_signed in *;
+      rewrite H1 in H;
+      process_keys_messages.
+    specialize (H0 _ _ Heq); split_ex; contra_map_lookup.
+  Qed.
+
+  Hint Resolve honestly_signed_message_in_key_heap.
 
   Lemma honest_labeled_step_message_queues_ok :
     forall {A B C} u_id suid cs cs' lbl (usrs usrs' : honest_users A) (adv adv' : user_data B)
@@ -1220,66 +1441,42 @@ Section UniverseLemmas.
   Proof.
     induction 1; inversion 2; inversion 6; intros; subst; try discriminate;
       eauto 2; autorewrite with find_user_keys; eauto;
-        clean_context.
+        clean_context; msg_queue_prop; specialize_msg_ok; eauto.
 
-    - assert (msg_honestly_signed (findUserKeys usrs') msg = true) by eauto.
+    eapply message_queues_ok_readd_user_same_queue;
+      clean_map_lookups; eauto.
 
-      match goal with
-      | [ OK : message_queues_ok _ ?us _ |- _ ] =>
+    unfold keys_and_permissions_good in *; split_ands; permission_heaps_prop.
+    msg_queue_prop.
+    econstructor; autorewrite with find_user_keys; eauto.
+    simpl.
+    eapply Forall_app; simpl; econstructor; eauto.
+    split; intros.
+    - unfold not; intros.
+      specialize (H0 _ _ H12).
+      split_ors; split_ands;
         match goal with
-        | [ H : us $? _ = Some _ |- _ ] => generalize (Forall_natmap_in_prop _ OK H); simpl; intros
-        | _ => let USR := fresh "USR"
-              in user_queue_lkup USR;
-                   do 3 (destruct USR as [?x USR]);
-                   generalize (Forall_natmap_in_prop _ OK USR); simpl; intros
-        end
-      end.
-      invert H0; split_ands.
-      msg_queue_prop; econstructor; eauto;
-        autorewrite with find_user_keys; eauto.
-      unfold message_queues_ok in *; rewrite Forall_natmap_forall in *; intros; eauto.
+        | [ H : permission_heap_good _ ?ks , H1 : ?ks $? _ = _ |- _ ] =>
+          specialize (H _ _ H1); split_ex; contra_map_lookup
+        end.
+    - assert (List.In cid mycs') by eauto.
+      split; eauto.
+      user_cipher_queues_prop; split; intros; contra_map_lookup.
 
-    - assert (message_queues_ok cs' usrs gks') as MQOK by assumption.
-      eapply message_queues_ok_readd_user_same_queue; clean_map_lookups; eauto.
+      unfold cipher_honestly_signed in *.
+      destruct msg; simpl in *;
+        encrypted_ciphers_prop;
+        intuition eauto;
+        try discriminate;
+        unfold message_no_adv_private;
+        intros;
+        simpl in *;
+        clean_context;
+        context_map_rewrites;
+        clean_map_lookups.
 
-      destruct rec_u; simpl in *.
-      eapply Forall_natmap_in_prop with (k:=rec_u_id) in MQOK; eauto; simpl in *.
-      econstructor; autorewrite with find_user_keys; eauto; simpl.
-      eapply Forall_app; econstructor; eauto.
-      intuition idtac.
-      + specialize (H0 _ _ H6).
-        unfold keys_and_permissions_good in *; split_ands.
-        eapply Forall_natmap_in_prop in H9; eauto; simpl in H9;
-          split_ors; split_ands;
-            match goal with
-            | [ H : permission_heap_good _ ?ks , H1 : ?ks $? _ = _ |- _ ] =>
-              specialize (H _ _ H1); split_ex; contra_map_lookup
-            end.
-      + unfold msg_honestly_signed in *.
-        assert (permission_heap_good gks' (findUserKeys usrs)); unfold keys_and_permissions_good in *; split_ands; eauto.
-        destruct msg; try discriminate; unfold honest_keyb in *; simpl in *; invert H6;
-          cases (findUserKeys usrs $? k); try discriminate;
-            specialize (H8 _ _ Heq); split_ex; contra_map_lookup.
-      + destruct msg; try discriminate;
-          unfold keys_and_permissions_good in *; split_ands;
-            eapply Forall_natmap_in_prop in H9; eauto;
-              simpl in *;
-              user_cipher_queues_prop;
-              match goal with
-              | [ H : msgCiphersSignedOk ?honk ?cphrs ?cipherMsg |- _ ] =>
-                assert (msgCiphersSignedOk honk cphrs cipherMsg) as MCSGN by assumption;
-                  unfold msgCiphersSignedOk in MCSGN;
-                  apply Forall_inv in MCSGN; unfold msgCipherOk in MCSGN; split_ands; split_ex
-              end; encrypted_ciphers_prop;
-                unfold msg_honestly_signed in *;
-                intuition contra_map_lookup;
-                repeat
-                  match goal with
-                  | [ H : honest_keyb ?honk ?kid = _ |- context [ honest_keyb ?honk ?kid] ] => rewrite H
-                  | [ |- context [ message_no_adv_private ] ] => unfold message_no_adv_private
-                  | [ |- _ /\ _ ] => intuition eauto
-                  end; simpl in *; clean_map_lookups; destruct p; eauto; intros.
-        exfalso; eauto.
+      destruct p; specialize_msg_ok; eauto; exfalso; eauto.
+
   Qed.
 
   Lemma merge_keys_addnl_honest :
@@ -1326,7 +1523,7 @@ Section UniverseLemmas.
     encrypted_ciphers_prop.
     econstructor; autorewrite with find_user_keys; simpl; eauto.
     rewrite Forall_natmap_forall; intros; eauto.
-    clear H34; msg_queue_prop; eauto.
+    msg_queue_prop; eauto.
   Qed.
 
   Lemma adv_step_adv_cipher_queue_ok :
@@ -1352,32 +1549,10 @@ Section UniverseLemmas.
    - invert H18; split_ands.
      rewrite in_app_iff in H; split_ors; eauto.
    - destruct (c_id ==n x); subst; clean_map_lookups; eauto.
-     invert H6; try contradiction; eauto.
-   - rewrite in_app_iff in H4; split_ors; eauto.
-     encrypted_ciphers_prop; eauto.
-     unfold adv_no_honest_keys in H23; specialize (H23 k__encid);
-       split_ors; split_ands; contra_map_lookup; contradiction.
+     invert H5; try contradiction; eauto.
    - destruct (c_id ==n x); subst; clean_map_lookups; eauto.
      invert H2; try contradiction; eauto.
   Qed.
-
-  (* Definition msg_signing_key {t} (msg : crypto t) : option key_identifier := *)
-  (*   match msg with *)
-  (*   | SignedCiphertext k _ _ => Some k *)
-  (*   | Signature _ k _ => Some k *)
-  (*   | _ => None *)
-  (*   end. *)
-
-  (* Definition message_queue_ok' (honestk : key_perms) (cs : ciphers) (msgs : queued_messages) (gks : keys) := *)
-  (*   Forall (fun sigm => match sigm with *)
-  (*                    | (existT _ _ m) => *)
-  (*                      (forall k kp, findKeysCrypto m $? k = Some kp -> gks $? k <> None) *)
-  (*                      /\ (forall k,   msg_signing_key m = Some k *)
-  (*                              -> honest_key honestk k *)
-  (*                              -> gks $? k <> None *)
-  (*                              /\ message_no_adv_private honestk m *)
-  (*                              /\ msgCiphersSignedOk honestk cs m) *)
-  (*                    end) msgs. *)
 
   (* Lemma not_in_cipherheap_not_in_mycs : *)
   (*   forall cs c_id honestk mycs, *)
@@ -1460,6 +1635,23 @@ Section UniverseLemmas.
   (*             unfold msgCiphersSignedOk; econstructor; intuition (simpl; eauto). *)
   (* Qed. *)
 
+  Lemma adv_cipher_in_cipher_heap :
+    forall {t} (msg : crypto t) adv_heap cs cid,
+      incl (findCiphers msg) adv_heap
+      -> adv_cipher_queue_ok cs adv_heap
+      -> msg_cipher_id msg = Some cid
+      -> exists c, cs $? cid = Some c.
+  Proof.
+    intros.
+    unfold msg_cipher_id, adv_cipher_queue_ok in *.
+    rewrite Forall_forall in H0.
+    destruct msg; try discriminate;
+      invert H1;
+      simpl in *;
+      assert (List.In cid adv_heap) as LIN by eauto;
+      specialize (H0 _ LIN); auto.
+  Qed.
+
   Lemma adv_step_message_queues_ok :
     forall {A B C} cs cs' lbl (usrs usrs' : honest_users A) (adv adv' : user_data B)
               gks gks' ks ks' qmsgs qmsgs' mycs mycs' bd bd',
@@ -1483,6 +1675,50 @@ Section UniverseLemmas.
     induction 1; inversion 1; inversion 10; intros; subst;
       eauto 2; try discriminate; eauto;
         clean_context.
+    
+    unfold message_queues_ok in *;
+      rewrite Forall_natmap_forall in *;
+      intros.
+
+    destruct (rec_u_id ==n k); subst; clean_map_lookups;
+      eauto;
+      autorewrite with find_user_keys;
+      simpl; eauto.
+
+    unfold message_queue_ok; eapply Forall_app.
+    unfold message_queue_ok in *; econstructor; eauto.
+    split; intros.
+    (* - specialize (H0 _ _ H); split_ors; split_ands; subst; eauto. *)
+    (*   specialize (H22 _ _ H0); unfold not; intros; split_ex; contra_map_lookup. *)
+    (*   specialize (H22 _ _ H0); unfold not; intros; split_ex; contra_map_lookup. *)
+    (* - assert (exists cid, msg_cipher_id msg = Some cid) by admit; split_ex. *)
+    (*   eapply adv_cipher_in_cipher_heap in H1; eauto; split_ex. *)
+    (*   assert (honest_key (findUserKeys usrs) k0) by admit. *)
+    (*   invert H5; specialize (H21 _ _ H6); split_ex. *)
+    (*   split; intros. *)
+    (*   + unfold not; intros; contra_map_lookup. *)
+
+    (*   + clear H20. *)
+    (*     assert (msgCipherOk cs' msg) by admit. *)
+    (*     unfold msgCipherOk, msg_cipher_id, msg_signing_key in H, H2, H8. *)
+    (*     destruct msg; try discriminate; split_ex; *)
+    (*       repeat match goal with *)
+    (*              | [ H : Some _ = Some _ |- _] => invert H *)
+    (*              end; clean_map_lookups; *)
+    (*         simpl in *; *)
+    (*         unfold message_no_adv_private, msgCiphersSignedOk; *)
+    (*         encrypted_ciphers_prop. *)
+
+    (*     * intuition (clean_map_lookups; eauto). *)
+    (*       econstructor; eauto. *)
+    (*       unfold msgCipherOk, msg_honestly_signed; eauto. *)
+          
+    (*     * intuition  (clean_map_lookups; eauto). *)
+    (*       ** destruct p; eauto; exfalso; eauto. *)
+    (*       ** destruct p; eauto; exfalso; eauto. *)
+    (*       ** econstructor; eauto. *)
+    (*          unfold msgCipherOk, msg_honestly_signed; eauto. *)
+    
   Admitted.
   
   Lemma adv_message_queue_ok_addnl_pubk :
@@ -1493,9 +1729,9 @@ Section UniverseLemmas.
       -> adv_message_queue_ok (honestk $k++ pubk) cs gks msgs.
   Proof.
     unfold adv_message_queue_ok; induction 1; intros; econstructor; eauto.
-    destruct x; split; intros; split_ands; eauto.
-    specialize (H _ _ H2); split_ands; subst.
-    intuition idtac.
+    destruct x; intuition eauto;
+      specialize (H _ _ H5); split_ands; eauto.
+
     apply merge_perms_split in H6; split_ors; eauto.
   Qed.
   
@@ -1525,8 +1761,8 @@ Section UniverseLemmas.
       eauto 2; autorewrite with find_user_keys; eauto;
         clean_context.
 
-    assert (msg_honestly_signed (findUserKeys usrs') msg = true) by eauto.
-    msg_queue_prop; eauto.
+    assert (msg_honestly_signed (findUserKeys usrs') cs' msg = true) by eauto.
+    msg_queue_prop; specialize_msg_ok; eauto.
   Qed.
 
   Lemma honest_labeled_step_adv_cipher_queue_ok :
@@ -1565,9 +1801,12 @@ Section UniverseLemmas.
     unfold adv_message_queue_ok in *; apply Forall_forall; intros.
     rewrite Forall_forall in H; specialize (H x); destruct x; intros.
     specialize (H H1); split_ands.
-    split; intros; eauto.
-    specialize (H _ _ H3).
+    intuition eauto;
+      specialize (H2 _ _ H4); split_ands; subst; eauto.
+
     destruct (k_id ==n k); subst; clean_map_lookups; try contradiction; intuition idtac.
+    destruct (k_id ==n k); subst; clean_map_lookups; eauto.
+    eapply H0; rewrite in_find_iff; unfold not; intros; contradiction.
   Qed.
 
   Lemma honest_silent_step_adv_cipher_queue_ok :
@@ -1603,9 +1842,10 @@ Section UniverseLemmas.
     unfold adv_message_queue_ok in *; apply Forall_forall; intros.
     rewrite Forall_forall in H; specialize (H x); destruct x; intros.
     specialize (H H1); split_ands.
-    split; intros; eauto.
-    specialize (H _ _ H3).
-    destruct (k_id ==n k); subst; clean_map_lookups; try contradiction; intuition idtac.
+    intuition eauto;
+      specialize (H2 _ _ H4); split_ands; eauto.
+
+    destruct (k_id ==n k); subst; clean_map_lookups; try contradiction.
   Qed.
 
   Hint Resolve adv_message_queue_ok_addnl_honestk_key adv_message_queue_ok_addnl_global_key.
@@ -1620,10 +1860,38 @@ Section UniverseLemmas.
     rewrite Forall_forall in *; intros.
     specialize (H0 _ H1).
     destruct x; split_ands.
-    split; eauto; intros.
-    destruct (c_id ==n c_id0); subst; clean_map_lookups; eauto.
-  Qed.
 
+    intuition eauto.
+    - destruct (c_id ==n cid); subst; clean_map_lookups; eauto.
+    - unfold findKeysCrypto in H4.
+      destruct c0; eauto; simpl in *.
+      + specialize (H2 _ _ H4); split_ands; eauto.
+      + specialize (H0 c_id0).
+        rewrite in_find_iff in H.
+        
+        destruct (c_id ==n c_id0); subst; clean_map_lookups; eauto.
+        cases (cs $? c_id0); eauto.
+        destruct c0; clean_map_lookups.
+        specialize (H2 _ _ H4); split_ands; eauto.
+    - unfold findKeysCrypto in H4; destruct c0; simpl in *; eauto.
+      * specialize (H2 _ _ H4); split_ands; eauto.
+      * destruct (c_id ==n c_id0); subst; clean_map_lookups; eauto.
+        ** assert (~ In c_id0 cs) by eauto; clean_map_lookups; context_map_rewrites.
+           specialize (H0 c_id0); exfalso; eauto.
+        ** cases (cs $? c_id0); clean_map_lookups.
+           destruct c0; clean_map_lookups.
+           specialize (H2 _ _ H4); split_ands; eauto.
+    - unfold findKeysCrypto in H4; destruct c0; simpl in *; eauto.
+      * specialize (H2 _ _ H4); split_ands; eauto.
+      * destruct (c_id ==n c_id0); subst; clean_map_lookups; eauto.
+        ** assert (~ In c_id0 cs) by eauto; clean_map_lookups; context_map_rewrites.
+           specialize (H0 c_id0); exfalso; eauto.
+        ** cases (cs $? c_id0); clean_map_lookups.
+           destruct c0; clean_map_lookups.
+           specialize (H2 _ _ H4); split_ands; eauto.
+    - destruct (c_id ==n c_id0); subst; clean_map_lookups; eauto.
+  Qed.
+           
   Hint Resolve adv_message_queue_ok_addnl_cipher.
 
   Lemma honest_silent_step_adv_message_queue_ok :
@@ -1707,8 +1975,7 @@ Section UniverseLemmas.
         autorewrite with find_user_keys; eauto;
           clean_context.
 
-    - assert (msg_honestly_signed (findUserKeys usrs') msg = true) by eauto.
-      msg_queue_prop;
+    - msg_queue_prop; specialize_msg_ok;
         unfold adv_no_honest_keys, message_no_adv_private in *;
         simpl in *;
         repeat
@@ -1716,14 +1983,14 @@ Section UniverseLemmas.
           | [ RW : honest_keyb ?honk ?kid = _ , H : if honest_keyb ?honk ?kid then _ else _ |- _] => rewrite RW in H
           | [ H : (forall k_id, findUserKeys _ $? k_id = None \/ _) |- (forall k_id, _) ] => intro KID; specialize (H KID)
           | [ |- context [ _ $k++ $0 ] ] => rewrite merge_keys_right_identity
-          | [ FK : findKeysCrypto ?msg $? ?kid = Some _, H : (forall k p, findKeysCrypto ?msg $? k = Some p -> _)
-              |- context [ _ $k++ findKeysCrypto ?msg $? ?kid] ] => specialize (H _ _ FK); split_ands; try simplify_key_merges1
-          | [ FK : findKeysCrypto ?msg $? ?kid = None |- context [ ?uks $k++ findKeysCrypto ?msg $? ?kid] ] =>
+          | [ FK : findKeysCrypto _ ?msg $? ?kid = Some _, H : (forall k p, findKeysCrypto _ ?msg $? k = Some p -> _)
+              |- context [ _ $k++ findKeysCrypto _ ?msg $? ?kid] ] => specialize (H _ _ FK); split_ands; try simplify_key_merges1
+          | [ FK : findKeysCrypto _ ?msg $? ?kid = None |- context [ ?uks $k++ findKeysCrypto _ ?msg $? ?kid] ] =>
             split_ors; split_ands; simplify_key_merges1
-          | [ H : (forall k p, findKeysCrypto ?msg $? k = Some p -> _)  |- context [ _ $k++ findKeysCrypto ?msg $? ?kid] ] =>
+          | [ H : (forall k p, findKeysCrypto _ ?msg $? k = Some p -> _)  |- context [ _ $k++ findKeysCrypto ?cs ?msg $? ?kid] ] =>
             match goal with
-            | [ H : findKeysCrypto msg $? kid = _ |- _ ] => fail 1
-            | _ => cases (findKeysCrypto msg $? kid)
+            | [ H : findKeysCrypto cs msg $? kid = _ |- _ ] => fail 1
+            | _ => cases (findKeysCrypto cs msg $? kid)
             end
           end; eauto.
 
@@ -1731,7 +1998,7 @@ Section UniverseLemmas.
 
     - unfold adv_no_honest_keys in *; intros.
       specialize (H18 k_id).
-      assert (findKeysCrypto msg $? k_id <> Some true) by eauto.
+      assert (findKeysCrypto cs' msg $? k_id <> Some true) by eauto.
       intuition idtac.
       right; right; split; eauto; intros.
 
@@ -1855,16 +2122,17 @@ Section UniverseLemmas.
       unfold adv_no_honest_keys in *; intros.
       specialize (H1 k_id); specialize (H18 k_id); split_ors; intuition idtac.
       right; right; intuition eauto.
-      eapply merge_perms_split in H4; split_ors; auto.
-      specialize (H2 _ _ H4); split_ands; contradiction.
+      eapply merge_perms_split in H8; split_ors; auto.
+      specialize (H4 _ _ H8); split_ands; contradiction.
 
     - assert (adv_no_honest_keys (findUserKeys usrs') (key_heap adv')) as ADV by assumption.
       specialize (ADV k__encid); split_ors; split_ands; try contradiction;
         encrypted_ciphers_prop; clean_map_lookups; intuition idtac;
         unfold adv_no_honest_keys; intros;
-          specialize (H21 k_id); clean_map_lookups; intuition idtac;
+          specialize (H20 k_id); clean_map_lookups; intuition idtac;
             right; right; split; eauto; intros;
-              eapply merge_perms_split in H10; split_ors; eauto;
+              eapply merge_perms_split in H10; split_ors;
+                try contradiction;
                 specialize (H17 _ _ H10); split_ex; split_ands; eauto.
 
     - eapply adv_no_honest_keys_after_new_adv_key; eauto.
@@ -1894,22 +2162,22 @@ Section UniverseLemmas.
     - eapply SigEncCipherAdvSignedOk; eauto.
       + unfold not; intros.
         cases (honestk $? k__s); cases (pubk $? k__s); simplify_key_merges1; clean_context; eauto.
-        specialize (H4 _ _ Heq0); split_ands; subst; clean_map_lookups; contradiction.
-        specialize (H4 _ _ Heq0); split_ands; subst; clean_map_lookups.
+        specialize (H3 _ _ Heq0); split_ands; subst; clean_map_lookups; contradiction.
+        specialize (H3 _ _ Heq0); split_ands; subst; clean_map_lookups.
 
-      + intros. specialize (H2 _ _ H5); split_ex; split_ands; eexists; split; eauto.
+      + intros. specialize (H2 _ _ H4); split_ex; split_ands; eexists; split; eauto.
         unfold not; intros.
         cases (honestk $? k); cases (pubk $? k); simplify_key_merges1; clean_context; eauto.
-        specialize (H4 _ _ Heq0); split_ands; subst; clean_map_lookups.
+        specialize (H3 _ _ Heq0); split_ands; subst; clean_map_lookups.
         assert (Some true <> Some true) by auto; contradiction.
         assert (Some true <> Some true) by auto; contradiction.
-        specialize (H4 _ _ Heq0); split_ands; subst; clean_map_lookups; eauto.
+        specialize (H3 _ _ Heq0); split_ands; subst; clean_map_lookups; eauto.
 
     - eapply SigEncCipherHonestSignedEncKeyHonestOk; eauto.
       + cases (pubk $? k__s); simplify_key_merges1; eauto.
       + cases (pubk $? k__e); simplify_key_merges1; eauto.
       + unfold keys_mine in *; intros.
-        specialize (H3 _ _ H6).
+        specialize (H3 _ _ H5).
         split_ors; split_ands; subst;
           cases (pubk $? k_id); simplify_key_merges1; eauto.
   Qed.
@@ -1950,19 +2218,15 @@ Section UniverseLemmas.
 
     - econstructor; eauto.
       assert (adv_no_honest_keys (findUserKeys usrs') (key_heap adv')) as ADV by assumption.
-      specialize (H21 k__signid).
+      specialize (H20 k__signid).
       econstructor; eauto.
       + unfold not; intros; split_ors; split_ands; contra_map_lookup; contradiction.
-      + intros. clear H21.
-        specialize (H4 _ _ H6); split_ors; split_ands; try discriminate.
-        specialize (H22 _ _ H4); split_ex; eexists.
+      + intros; clear H20.
+        specialize (H4 _ _ H5); destruct H4; split_ands; subst; eauto.
+        specialize (H21 _ _ H4); split_ex; eexists.
         specialize (ADV k); intuition eauto; contra_map_lookup; subst; eauto.
-        specialize (H22 _ _ H4); split_ex; eexists.
+        specialize (H21 _ _ H4); split_ex; eexists.
         specialize (ADV k); intuition eauto; contra_map_lookup; subst; eauto.
-      + intros.
-        destruct (c_id ==n cid); subst; clean_map_lookups; eauto.
-        specialize (H5 _ H6).
-        unfold adv_cipher_queue_ok in H23; rewrite Forall_forall in H23; eauto.
     - econstructor; eauto.
       specialize (H17 k_id).
       eapply SigCipherNotHonestOk; eauto.
@@ -1982,6 +2246,7 @@ Section SingleAdversarySimulates.
    *   or, prove an appended simulation relation, but I am not sure how to generically express this
    *)
   Hint Resolve accepted_safe_msg_pattern_honestly_signed.
+  Hint Resolve encrypted_ciphers_ok_addnl_cipher.
 
   Section RealWorldLemmas.
     Import RealWorld.
@@ -2042,8 +2307,8 @@ Section SingleAdversarySimulates.
          adv_key_not_honestk.
 
     Lemma user_cipher_queue_cleaned_users_nochange :
-      forall {A} (usrs : honest_users A) honestk u_id,
-        user_cipher_queue (clean_users honestk usrs) u_id
+      forall {A} (usrs : honest_users A) honestk cs u_id,
+        user_cipher_queue (clean_users honestk cs usrs) u_id
         = user_cipher_queue usrs u_id.
     Proof.
       unfold user_cipher_queue, clean_users; simpl; intros.
@@ -2057,7 +2322,7 @@ Section SingleAdversarySimulates.
         -> user_data' =
             {| key_heap := clean_key_permissions (findUserKeys U.(users)) user_data.(key_heap)
              ; protocol := user_data.(protocol)
-             ; msg_heap := clean_messages (findUserKeys U.(users)) user_data.(msg_heap)
+             ; msg_heap := clean_messages (findUserKeys U.(users)) U.(all_ciphers) user_data.(msg_heap)
              ; c_heap   := user_data.(c_heap) |}
         -> (strip_adversary U).(s_users) $? u_id = Some user_data'.
     Proof.
@@ -2070,52 +2335,56 @@ Section SingleAdversarySimulates.
     Hint Resolve user_in_univ_user_in_stripped_univ.
 
     Lemma prop_in_adv_message_queues_still_good_after_cleaning :
-      forall msgs honestk P,
+      forall msgs honestk cs P,
         Forall P msgs
-        -> Forall P (clean_messages honestk msgs).
+        -> Forall P (clean_messages honestk cs msgs).
     Proof.
       induction msgs; intros; eauto.
       invert H.
       unfold clean_messages; simpl.
-      cases (msg_filter honestk a); eauto.
+      cases (msg_filter honestk cs a); eauto.
     Qed.
 
     Hint Resolve prop_in_adv_message_queues_still_good_after_cleaning.
 
+    Hint Resolve honest_cipher_filter_fn_true_honest_signing_key.
+    Hint Extern 1 (honest_key _ _) => process_keys_messages.
+    Hint Resolve
+         msg_honestly_signed_after_without_cleaning
+         msg_honestly_signed_before_after_cleaning.
+                                               
     Lemma msgCiphersSigned_before_clean_ciphers' :
       forall (msgs : queued_messages) honestk cs,
-        Forall (fun sigm => match sigm with (existT _ _ m) => msgCipherOk (clean_ciphers honestk cs) m /\ msg_honestly_signed honestk m = true end) msgs
-        -> Forall (fun sigm => match sigm with (existT _ _ m) => msgCipherOk cs m /\ msg_honestly_signed honestk m = true end) msgs.
+        Forall (fun sigm => match sigm with (existT _ _ m) => msg_honestly_signed honestk (clean_ciphers honestk cs) m = true end) msgs
+        -> Forall (fun sigm => match sigm with (existT _ _ m) => msg_honestly_signed honestk cs m = true end) msgs.
     Proof.
       induction 1; econstructor; eauto.
-      unfold msgCipherOk in *.
-      destruct x; intuition idtac.
-      destruct c; eauto; split_ex;
-        match goal with
-        | [ H : clean_ciphers _ _ $? _ = Some _ |- _ ] => rewrite <- find_mapsto_iff in H; rewrite clean_ciphers_mapsto_iff in H
-        end;
-        repeat eexists; split_ands;
-          rewrite <- find_mapsto_iff; eauto.
+      destruct x; intuition eauto.
     Qed.
 
     Hint Resolve clean_ciphers_keeps_honest_cipher.
 
     Lemma msgCiphersSigned_after_clean_ciphers' :
-      forall (msgs : queued_messages) honestk cs,
-        Forall (fun sigm => match sigm with (existT _ _ m) => msgCipherOk cs m /\ msg_honestly_signed honestk m = true end) msgs
-        -> Forall (fun sigm => match sigm with (existT _ _ m) => msgCipherOk (clean_ciphers honestk cs) m /\ msg_honestly_signed honestk m = true end) msgs.
+      forall (msgs : queued_messages) honestk honestk' cs,
+        Forall (fun sigm => match sigm with (existT _ _ m) => msg_honestly_signed honestk cs m = true end) msgs
+        -> (forall k_id, honestk $? k_id = Some true -> honestk' $? k_id = Some true)
+        -> Forall (fun sigm => match sigm with (existT _ _ m) => msg_honestly_signed honestk' (clean_ciphers honestk cs) m = true end) msgs.
     Proof.
       induction 1; econstructor; eauto.
-      unfold msgCipherOk in *.
-      destruct x; intuition idtac.
-      destruct c; eauto; split_ex.
-      repeat eexists; eauto.
+      destruct x.
+      eapply msg_honestly_signed_before_after_cleaning in H.
+      unfold msg_honestly_signed in *.
+      cases ( msg_signing_key (clean_ciphers honestk cs) c ); try discriminate.
+      unfold honest_keyb in *.
+      cases (honestk $? k); try discriminate; destruct b; try discriminate.
+      specialize (H1 _ Heq0); rewrite H1; trivial.
     Qed.
 
     Lemma msgCiphersSigned_after_clean_ciphers :
-      forall {t} (msg : crypto t) honestk cs,
+      forall {t} (msg : crypto t) honestk honestk' cs,
         msgCiphersSignedOk honestk cs msg
-        -> msgCiphersSignedOk honestk (clean_ciphers honestk cs) msg.
+        -> (forall k_id, honestk $? k_id = Some true -> honestk' $? k_id = Some true)
+        -> msgCiphersSignedOk honestk' (clean_ciphers honestk cs) msg.
     Proof.
       intros; eapply msgCiphersSigned_after_clean_ciphers'; eauto.
     Qed.
@@ -2224,8 +2493,8 @@ Section SingleAdversarySimulates.
       forall {A} (usrs : honest_users A) honestk honestk' cs,
         user_cipher_queues_ok cs honestk usrs
         -> honestk = findUserKeys usrs
-        -> honestk' = findUserKeys (clean_users honestk usrs)
-        -> user_cipher_queues_ok (clean_ciphers honestk cs) honestk' (clean_users honestk usrs).
+        -> honestk' = findUserKeys (clean_users honestk cs usrs)
+        -> user_cipher_queues_ok (clean_ciphers honestk cs) honestk' (clean_users honestk cs usrs).
     Proof.
       unfold user_cipher_queues_ok; intros.
       pose proof (clean_users_no_change_honestk usrs).
@@ -2236,51 +2505,128 @@ Section SingleAdversarySimulates.
       eapply user_cipher_queue_ok_after_cleaning; auto.
     Qed.
 
+    Lemma msg_honestly_signed_cipher_honestly_signed :
+      forall {t} (msg : crypto t) honestk c cs cid,
+        msg_honestly_signed honestk cs msg = true
+        -> msg_cipher_id msg = Some cid
+        -> cs $? cid = Some c
+        (* -> msgCipherOk cs msg *)
+        -> honest_keyb honestk (cipher_signing_key c) = true.
+    Proof.
+      intros.
+      unfold msg_honestly_signed, msg_cipher_id in *;
+        unfold cipher_signing_key;
+        destruct msg; simpl in *; try discriminate; split_ex;
+          invert H0;
+          rewrite H1 in H;
+          destruct c;
+          try discriminate;
+          eauto.
+    Qed.
+
+    Hint Resolve msg_honestly_signed_cipher_honestly_signed.
+
+    (* Lemma msgCipherOk_honest_msgCipherOk_cleaned : *)
+    (*   forall {t} cs (msg : crypto t) honestk, *)
+    (*     msgCipherOk cs msg *)
+    (*     -> msg_honestly_signed honestk msg = true *)
+    (*     -> msgCipherOk (clean_ciphers honestk cs) msg. *)
+    (* Proof. *)
+    (*   intros. *)
+    (*   unfold msgCipherOk, msg_honestly_signed in *. *)
+    (*   destruct msg; try discriminate; *)
+    (*     split_ex; eauto. *)
+    (* Qed. *)
+
+    (* Hint Resolve msgCipherOk_honest_msgCipherOk_cleaned. *)
+
+    Lemma findKeysCrypto_ok_clean_global_keys :
+      forall {t} (msg : crypto t) cs gks honestk,
+        (forall k kp, findKeysCrypto cs msg $? k = Some kp -> gks $? k <> None)
+        -> message_no_adv_private honestk cs msg
+        -> (forall k kp, findKeysCrypto cs msg $? k = Some kp -> clean_keys honestk gks $? k <> None).
+    Proof.
+      unfold message_no_adv_private; intros.
+      specialize (H _ _ H1).
+      specialize (H0 _ _ H1); split_ands; subst.
+      cases (gks $? k); try contradiction.
+      unfold not; intros.
+      erewrite clean_keys_keeps_honest_key in H2; eauto.
+    Qed.
+    
+    Hint Resolve findKeysCrypto_ok_clean_global_keys.
+
+    Lemma msg_signing_key_same_after_cleaning :
+      forall {t} (msg : crypto t) cs honestk k1 k2,
+        msg_signing_key cs msg = Some k1
+        -> msg_signing_key (clean_ciphers honestk cs) msg = Some k2
+        -> k1 = k2.
+    Proof.
+      unfold msg_signing_key; intros.
+      destruct msg; try discriminate.
+      - cases (cs $? c_id); cases (clean_ciphers honestk cs $? c_id); try discriminate.
+        rewrite <- find_mapsto_iff in Heq0; rewrite clean_ciphers_mapsto_iff in Heq0; rewrite find_mapsto_iff in Heq0;
+          split_ands; clean_map_lookups.
+        destruct c0; try discriminate; clean_context; trivial.
+    Qed.
+
     Lemma message_queue_ok_after_cleaning :
       forall msgs honestk honestk' cs gks,
         message_queue_ok honestk cs msgs gks
         -> encrypted_ciphers_ok honestk cs gks
         -> (forall k_id, honestk $? k_id = Some true -> honestk' $? k_id = Some true)
         -> message_queue_ok honestk' (clean_ciphers honestk cs)
-                           (clean_messages honestk msgs) (clean_keys honestk gks).
+                           (clean_messages honestk cs msgs) (clean_keys honestk gks).
     Proof.
       intros; unfold message_queue_ok in *; rewrite Forall_forall in *; intros.
-      destruct x; simpl in *; intros.
-
+      specialize (H x).
       apply filter_In in H2; split_ands.
-      specialize (H _ H2); simpl in *.
-      unfold msg_honestly_signed in H3; split_ands.
+      specialize (H H2); simpl in *; split_ands.
+      destruct x; split_ands; simpl in *; specialize_msg_ok.
+      cases (gks $? x1 ); try contradiction.
+      cases (cs $? x0); try contradiction.
+      clear H4 H7.
 
-      split; intros.
-      - specialize (H _ _ H5).
-        unfold not; intros.
-        cases (gks $? k); try contradiction; clear H.
-        destruct c; simpl in *; try discriminate; split_ands.
-        assert (Some k1 = Some k1) as SK by trivial; specialize (H4 _ SK); split_ands.
-        assert (honest_key honestk k1) as HK by (rewrite <- honest_key_honest_keyb in *; auto);
-          specialize (H4 HK); split_ands.
-        unfold message_no_adv_private, msgCiphersSignedOk, msgCipherOk in *; simpl in *.
-        specialize (H4 _ _ H5); split_ands; try discriminate; subst.
-        eapply clean_keys_keeps_honest_key with (honestk := honestk) in Heq; eauto; contra_map_lookup.
+      split; eauto; intros.
 
-      - specialize_msg_queue_ok.
-        split; intros.
-        + cases (gks $? k); try contradiction; clear H4.
-          unfold not; intros.
-          eapply clean_keys_inv' in H4; eauto.
-          unfold honest_key_filter_fn in *.
-          assert (honest_keyb honestk k = false) by (unfold honest_keyb; auto).
-          unfold msg_signing_key in *; destruct c; clean_map_lookups;
-            match goal with
-            | [ H1 : honest_keyb ?honk ?k = true, H2 : honest_keyb ?honk ?k = false |- _ ] => rewrite H1 in H2; discriminate H2
-            end.
-        + destruct H7; unfold honest_keyb, msg_signing_key in *; invert H5.
-          destruct c; try discriminate; invert H9;
-            assert (honest_key honestk k) as HK
-              by (constructor; cases (honestk $? k); try discriminate; destruct b; try discriminate; trivial);
-            specialize (H6 HK); unfold message_no_adv_private in *;
-              intuition eauto using msgCiphersSigned_cleaned_honestk;
-              specialize (H5 _ _ H6); split_ands; auto.
+      unfold msg_signing_key,msg_cipher_id in H5, H6; destruct c; try discriminate; clean_context.
+      rewrite Heq0 in H5; clean_context.
+      simpl in *. context_map_rewrites.
+      cases (clean_ciphers honestk cs $? x0); try discriminate.
+      rewrite <- find_mapsto_iff in Heq1; rewrite clean_ciphers_mapsto_iff in Heq1; rewrite find_mapsto_iff in Heq1; split_ands;
+        clean_map_lookups.
+      destruct c; try discriminate.
+      specialize (H _ _ H4); simpl in *.
+      unfold message_no_adv_private in H8; simpl in *; context_map_rewrites.
+      specialize (H8 _ _ H4); split_ands; subst.
+      unfold not; intros.
+      cases (gks $? k0); try contradiction.
+      eapply clean_keys_inv' in H7; unfold honest_key_filter_fn in *; context_map_rewrites; try discriminate; reflexivity.
+                                                                                                                      
+      assert (x1 = k0) by eauto using msg_signing_key_same_after_cleaning; subst.
+      rewrite H6 in H7; clean_context.
+      eapply clean_keys_keeps_honest_key with (honestk := honestk) in Heq.
+      2:unfold honest_key_filter_fn; invert H9; context_map_rewrites; trivial.
+
+      split.
+      unfold not; intros; contra_map_lookup.
+
+      split.
+      unfold msg_signing_key,msg_cipher_id in H5, H6; destruct c; try discriminate; clean_context.
+      rewrite Heq0 in H5; clean_context.
+      simpl in *. context_map_rewrites.
+      cases (clean_ciphers honestk cs $? cid); try discriminate.
+
+      unfold message_no_adv_private in *; intros.
+
+      split; eauto; intros.
+
+      assert (findKeysCrypto cs c $? k1 = Some p).
+      unfold findKeysCrypto in H11; unfold findKeysCrypto; destruct c; try discriminate.
+      cases (clean_ciphers honestk cs $? c_id); try discriminate.
+      rewrite <- find_mapsto_iff in Heq1; rewrite clean_ciphers_mapsto_iff in Heq1; rewrite find_mapsto_iff in Heq1; split_ands.
+      context_map_rewrites; eauto.
+      specialize (H8 _ _ H12); split_ands; eauto.
     Qed.
 
     Lemma message_queues_ok_after_cleaning :
@@ -2288,7 +2634,7 @@ Section SingleAdversarySimulates.
         message_queues_ok cs usrs gks
         -> honestk = findUserKeys usrs
         -> encrypted_ciphers_ok honestk cs gks
-        -> message_queues_ok (clean_ciphers honestk cs) (clean_users honestk usrs) (clean_keys honestk gks).
+        -> message_queues_ok (clean_ciphers honestk cs) (clean_users honestk cs usrs) (clean_keys honestk gks).
     Proof.
       unfold message_queues_ok; intros.
       pose proof (clean_users_no_change_honestk usrs).
@@ -2300,14 +2646,14 @@ Section SingleAdversarySimulates.
     Qed.
 
     Lemma adv_no_honest_keys_after_cleaning :
-      forall {A} (usrs : honest_users A) honestk honestk' adv_keys,
+      forall {A} (usrs : honest_users A) honestk honestk' cs adv_keys,
         adv_no_honest_keys honestk adv_keys
         -> honestk = findUserKeys usrs
-        -> honestk' = findUserKeys (clean_users honestk usrs)
+        -> honestk' = findUserKeys (clean_users honestk cs usrs)
         -> adv_no_honest_keys honestk' (clean_key_permissions honestk adv_keys).
     Proof.
       unfold adv_no_honest_keys; intros.
-      pose proof (findUserKeys_clean_users_correct usrs); subst.
+      pose proof (findUserKeys_clean_users_correct usrs cs k_id); subst.
       repeat
         match goal with
         | [ K : NatMap.key, H : (forall k : NatMap.key, _) |- _ ] => specialize (H K)
@@ -2351,13 +2697,13 @@ Section SingleAdversarySimulates.
          not_in_ciphers_not_in_cleaned_ciphers.
 
     Lemma cipher_message_keys_already_in_honest :
-      forall {A t} (msg : crypto t) (usrs : honest_users A) honestk cs c_id k__s k__e gks,
+      forall {A t} (msg : message t) (usrs : honest_users A) honestk cs c_id k__s k__e gks,
         honestk = findUserKeys usrs
         -> cs $? c_id = Some (SigEncCipher k__s k__e msg)
         -> honest_key honestk k__s
         -> honest_key honestk k__e
         -> encrypted_ciphers_ok honestk cs gks
-        -> honestk $k++ findKeysCrypto msg = honestk.
+        -> honestk $k++ findKeysMessage msg = honestk.
     Proof.
       intros.
       invert H1; invert H2.
@@ -2440,27 +2786,39 @@ Section SingleAdversarySimulates.
         (* permission_heap_good gks honestk *)
            message_queue_ok honestk cs msgs gks
         -> ~ In k_id gks
-        -> clean_messages (honestk $+ (k_id, true)) msgs = clean_messages honestk msgs.
+        -> clean_messages (honestk $+ (k_id, true)) cs msgs = clean_messages honestk cs msgs.
     Proof.
       induction msgs; intros; eauto; simpl.
-      case_eq (msg_filter honestk a); intros.
-      - assert (msg_filter (honestk $+ (k_id,true)) a = true) by
+      case_eq (msg_filter honestk cs a); intros.
+      - assert (msg_filter (honestk $+ (k_id,true)) cs a = true).
             (unfold msg_filter in *; destruct a; unfold msg_honestly_signed in *; destruct c; try discriminate;
-             unfold honest_keyb in *;
-             match goal with
-             | [ |- context [ _ $+ (?k1,_) $? ?k2]] => destruct (k1 ==n k2); subst; clean_map_lookups; eauto
-             end).
+             unfold honest_keyb in *; simpl in *;
+             repeat
+               match goal with
+               | [ H : context [ match cs $? ?cid with _ => _ end ] |- _ ] => cases (cs $? cid); try discriminate
+               | [ H : context [ match ?c with _ => _ end ] |- _ ] => is_var c; idtac c; destruct c; try discriminate
+               | [ |- context [ _ $+ (?k1,_) $? ?k2]] => destruct (k1 ==n k2); subst; clean_map_lookups; eauto
+               end).
         rewrite H2; invert H; erewrite IHmsgs; eauto.
 
       - invert H; destruct a; simpl in *; split_ands.
-        assert (msg_honestly_signed (honestk $+ (k_id,true)) c = false).
+        assert (msg_honestly_signed (honestk $+ (k_id,true)) cs c = false).
         unfold  msg_honestly_signed in *; destruct c; try discriminate;
           unfold honest_keyb, msg_signing_key in *; trivial;
-            match goal with
-            | [ |- context [ _ $+ (?k1,_) $? ?k2]] =>
-              assert (Some k2 = Some k2) as SK by trivial; specialize (H2 _ SK); split_ands;
-                destruct (k1 ==n k2); subst; clean_map_lookups; eauto; contradiction
-            end.
+            repeat
+              match goal with
+              | [ H : context [ match cs $? ?cid with _ => _ end ] |- _ ] => cases (cs $? cid); try discriminate
+              | [ H : context [ match ?c with _ => _ end ] |- _ ] => is_var c; destruct c; try discriminate
+              | [ |- context [ _ $+ (?k1,_) $? ?k2]] =>
+                idtac 1;
+                  assert (Some k2 = Some k2) as SK by trivial
+                  (* ; specialize (H2 _ _ SK); split_ands *)
+                  (* destruct (k1 ==n k2); subst; clean_map_lookups; eauto; contradiction *)
+              end; eauto; clean_context.
+        assert (Some (cipher_signing_key c) = Some (cipher_signing_key c)) as CSK by trivial.
+        assert (msg_cipher_id (@SignedCiphertext t0 c_id) = Some c_id) as MC by trivial.
+        specialize (H2 _ _ CSK MC); split_ands.
+        destruct (k_id ==n cipher_signing_key c); subst; clean_map_lookups; eauto; contradiction.
         rewrite H3; eauto.
     Qed.
 
@@ -2569,7 +2927,7 @@ Section SingleAdversarySimulates.
         -> honestk = findUserKeys usrs
         -> message_queues_ok cs usrs gks
         -> keys_and_permissions_good gks usrs adv_heap
-        -> clean_users (honestk $+ (k_id, true)) usrs = clean_users honestk usrs.
+        -> clean_users (honestk $+ (k_id, true)) cs usrs = clean_users honestk cs usrs.
     Proof.
       intros; subst.
       apply map_eq_Equal; unfold Equal; intros.
@@ -2615,6 +2973,31 @@ Section SingleAdversarySimulates.
       (*                         (usrs__s', clean_adv adv' (findUserKeys usrs) b, cs__s', clean_keys honestk' gks', *)
       (*                          clean_key_permissions honestk' ks', clean_messages honestk' qmsgs', mycs', cmd'). *)
 
+    Lemma honestly_signed_message_accepted_by_pattern_same_after_cleaning :
+      forall {t} (msg : crypto t) cs pat honestk,
+        msg_accepted_by_pattern cs pat msg
+        -> msg_honestly_signed honestk cs msg = true
+        -> msg_accepted_by_pattern (clean_ciphers honestk cs) pat msg.
+    Proof.
+      intros.
+      unfold msg_honestly_signed in *.
+      invert H; econstructor; simpl in *; context_map_rewrites; eauto.
+    Qed.
+    
+    Lemma message_not_accepted_by_pattern_same_after_cleaning :
+      forall {t} (msg : crypto t) cs pat honestk,
+        ~ msg_accepted_by_pattern cs pat msg
+        -> ~ msg_accepted_by_pattern (clean_ciphers honestk cs) pat msg.
+    Proof.
+      unfold not; intros; apply H.
+      invert H0; econstructor;
+        rewrite <- find_mapsto_iff, clean_ciphers_mapsto_iff, find_mapsto_iff in H4; split_ands; eauto.
+    Qed.
+
+    Hint Resolve
+         honestly_signed_message_accepted_by_pattern_same_after_cleaning
+         message_not_accepted_by_pattern_same_after_cleaning.
+    
     Lemma honest_silent_step_advuniv_implies_honest_or_no_step_origuniv :
       forall {A B C} u_id suid cs cs' lbl (usrs usrs' : honest_users A) (adv adv' : user_data B)
                 gks gks' ks ks' qmsgs qmsgs' mycs mycs' bd bd' (b: B),
@@ -2623,7 +3006,7 @@ Section SingleAdversarySimulates.
         -> forall (cmd : user_cmd C) cs__s usrs__s honestk,
           honestk = findUserKeys usrs
           -> cs__s = clean_ciphers honestk cs
-          -> usrs__s = clean_users honestk usrs
+          -> usrs__s = clean_users honestk cs usrs
           -> bd = (usrs, adv, cs, gks, ks, qmsgs, mycs, cmd)
           -> encrypted_ciphers_ok honestk cs gks
           -> user_cipher_queues_ok cs honestk usrs
@@ -2637,20 +3020,20 @@ Section SingleAdversarySimulates.
                   -> usrs'' = usrs' $+ (u_id, {| key_heap := ks' ; msg_heap := qmsgs' ; protocol := cmdc' ; c_heap := mycs' |})
                   -> honestk' = findUserKeys usrs''
                   -> cs__s' = clean_ciphers honestk' cs'
-                  -> usrs__s' = clean_users honestk' usrs'
+                  -> usrs__s' = clean_users honestk' cs' usrs'
                   -> encrypted_ciphers_ok honestk' cs' gks'
                   -> step_user lbl suid
                               (usrs__s, clean_adv adv honestk b, cs__s, clean_keys honestk gks,
-                               clean_key_permissions honestk ks, clean_messages honestk qmsgs, mycs, cmd)
+                               clean_key_permissions honestk ks, clean_messages honestk cs qmsgs, mycs, cmd)
                               (usrs__s', clean_adv adv' honestk' b, cs__s', clean_keys honestk' gks',
-                               clean_key_permissions honestk' ks', clean_messages honestk' qmsgs', mycs', cmd')
+                               clean_key_permissions honestk' ks', clean_messages honestk' cs' qmsgs', mycs', cmd')
                   \/ (usrs__s, clean_adv adv honestk b, cs__s, clean_keys honestk gks,
-                     clean_key_permissions honestk ks, clean_messages honestk qmsgs, mycs, cmd)
-                    = (clean_users honestk' usrs', clean_adv adv' honestk' b, cs__s', clean_keys honestk' gks',
-                       clean_key_permissions honestk' ks', clean_messages honestk' qmsgs', mycs', cmd').
+                     clean_key_permissions honestk ks, clean_messages honestk cs qmsgs, mycs, cmd)
+                    = (clean_users honestk' cs' usrs', clean_adv adv' honestk' b, cs__s', clean_keys honestk' gks',
+                       clean_key_permissions honestk' ks', clean_messages honestk' cs' qmsgs', mycs', cmd').
     Proof.
       induction 1; inversion 5; inversion 5; intros; subst; clean_context;
-        autorewrite with find_user_keys;
+        autorewrite with find_user_keys in *;
         try solve [ left; econstructor; eauto; user_cipher_queues_prop; eauto; try solve_clean_keys_clean_key_permissions ].
 
       - remember (findUserKeys usrs) as honestk.
@@ -2658,8 +3041,8 @@ Section SingleAdversarySimulates.
         remember (findUserKeys usrs'') as honestk'.
         remember (clean_ciphers honestk cs) as cs__s.
         remember (clean_ciphers honestk' cs') as cs__s'.
-        remember (clean_users honestk usrs) as usrs__s.
-        remember (clean_users honestk' usrs') as usrs__s'.
+        remember (clean_users honestk cs usrs) as usrs__s.
+        remember (clean_users honestk' cs' usrs') as usrs__s'.
         assert (@Silent action = Silent) as SIL by trivial.
         assert ((usrs,adv,cs,gks,ks,qmsgs,mycs,cmd1)=(usrs,adv,cs,gks,ks,qmsgs,mycs,cmd1)) as bd1 by trivial.
         assert ((usrs',adv',cs',gks',ks',qmsgs',mycs',cmd1')=(usrs',adv',cs',gks',ks',qmsgs',mycs',cmd1')) as bd1' by trivial.
@@ -2688,61 +3071,61 @@ Section SingleAdversarySimulates.
         + left; econstructor; eauto.
         + right; unfold clean_adv; simpl; inversion H1; subst. f_equal.
 
-      - cases (msg_honestly_signed (findUserKeys usrs') msg).
+      - cases (msg_honestly_signed (findUserKeys usrs') cs' msg).
         + left. econstructor; eauto.
           unfold clean_messages, msg_filter; simpl; rewrite Heq; eauto.
         + right; simpl; rewrite Heq; f_equal.
+          
+      (* - clear H14; encrypted_ciphers_prop. *)
+      (*     autorewrite with find_user_keys in *. *)
+      (*   * eapply findUserKeys_has_private_key_of_user in H36; eauto; contradiction. *)
+      (*   * left; econstructor; eauto; try solve_clean_keys_clean_key_permissions. *)
+      (*     unfold keys_mine; intros. *)
+      (*     specialize (H15 _ _ H6); split_ands; subst. *)
+      (*     specialize (H4 _ _ H6); split_ors; split_ands; eauto. *)
+      (*     ** left; apply clean_key_permissions_keeps_honest_permission; eauto; unfold honest_perm_filter_fn; context_map_rewrites; trivial. *)
+      (*     ** right; intuition idtac; *)
+      (*          apply clean_key_permissions_keeps_honest_permission; eauto; unfold honest_perm_filter_fn; context_map_rewrites; trivial. *)
 
-      - clear H14; encrypted_ciphers_prop;
-          autorewrite with find_user_keys in *.
-        * eapply findUserKeys_has_private_key_of_user in H36; eauto; contradiction.
-        * left; econstructor; eauto; try solve_clean_keys_clean_key_permissions.
-          unfold keys_mine; intros.
-          specialize (H15 _ _ H6); split_ands; subst.
-          specialize (H4 _ _ H6); split_ors; split_ands; eauto.
-          ** left; apply clean_key_permissions_keeps_honest_permission; eauto; unfold honest_perm_filter_fn; context_map_rewrites; trivial.
-          ** right; intuition idtac;
-               apply clean_key_permissions_keeps_honest_permission; eauto; unfold honest_perm_filter_fn; context_map_rewrites; trivial.
+      (* - autorewrite with find_user_keys in *. *)
+      (*   assert (findUserKeys usrs' $? k__encid = Some true) by eauto 2. *)
+      (*   clear H41. *)
+      (*   user_cipher_queues_prop. encrypted_ciphers_prop. *)
+      (*   rewrite merge_keys_addnl_honest; eauto. *)
+      (*   econstructor; econstructor; eauto; try solve_clean_keys_clean_key_permissions. *)
 
-      - autorewrite with find_user_keys in *.
-        assert (findUserKeys usrs' $? k__encid = Some true) by eauto 2.
-        clear H41.
-        user_cipher_queues_prop. encrypted_ciphers_prop.
-        rewrite merge_keys_addnl_honest; eauto.
-        econstructor; econstructor; eauto; try solve_clean_keys_clean_key_permissions.
+      (* - autorewrite with find_user_keys in *. *)
+      (*   msg_queue_prop. *)
+      (*   keys_and_permissions_prop. *)
 
-      - autorewrite with find_user_keys in *.
-        msg_queue_prop.
-        keys_and_permissions_prop.
+      (*   erewrite clean_users_new_honest_key_idempotent *)
+      (*          , clean_ciphers_new_honest_key_idempotent *)
+      (*          , clean_messages_new_honest_key_idempotent *)
+      (*          , clean_adv_new_honest_key_idempotent *)
+      (*          , clean_key_permissions_new_honest_key *)
+      (*   ; eauto. *)
 
-        erewrite clean_users_new_honest_key_idempotent
-               , clean_ciphers_new_honest_key_idempotent
-               , clean_messages_new_honest_key_idempotent
-               , clean_adv_new_honest_key_idempotent
-               , clean_key_permissions_new_honest_key
-        ; eauto.
+      (*   left; econstructor; eauto. *)
+      (*   eapply clean_keys_adds_no_keys; auto. *)
+      (*   cases (ks $? k_id); clean_map_lookups; eauto. *)
+      (*   specialize (H4 _ _ Heq); split_ex; contra_map_lookup. *)
 
-        left; econstructor; eauto.
-        eapply clean_keys_adds_no_keys; auto.
-        cases (ks $? k_id); clean_map_lookups; eauto.
-        specialize (H4 _ _ Heq); split_ex; contra_map_lookup.
+      (* - autorewrite with find_user_keys in *. *)
+      (*   msg_queue_prop. *)
+      (*   keys_and_permissions_prop. *)
 
-      - autorewrite with find_user_keys in *.
-        msg_queue_prop.
-        keys_and_permissions_prop.
+      (*   erewrite clean_users_new_honest_key_idempotent *)
+      (*          , clean_ciphers_new_honest_key_idempotent *)
+      (*          , clean_messages_new_honest_key_idempotent *)
+      (*          , clean_adv_new_honest_key_idempotent *)
+      (*          , clean_key_permissions_new_honest_key *)
+      (*   ; eauto. *)
 
-        erewrite clean_users_new_honest_key_idempotent
-               , clean_ciphers_new_honest_key_idempotent
-               , clean_messages_new_honest_key_idempotent
-               , clean_adv_new_honest_key_idempotent
-               , clean_key_permissions_new_honest_key
-        ; eauto.
-
-        left; econstructor; eauto.
-        eapply clean_keys_adds_no_keys; auto.
-        cases (ks $? k_id); clean_map_lookups; eauto.
-        specialize (H4 _ _ Heq); split_ex; contra_map_lookup.
-    Qed.
+      (*   left; econstructor; eauto. *)
+      (*   eapply clean_keys_adds_no_keys; auto. *)
+      (*   cases (ks $? k_id); clean_map_lookups; eauto. *)
+      (*   specialize (H4 _ _ Heq); split_ex; contra_map_lookup. *)
+    Admitted.
 
     Lemma honest_cipher_filter_fn_nochange_pubk :
       forall honestk pubk k v,
@@ -2752,15 +3135,10 @@ Section SingleAdversarySimulates.
     Proof.
       unfold honest_cipher_filter_fn; intros;
         unfold cipher_honestly_signed;
-        cases v; unfold honest_keyb; simpl.
-
-      - cases (honestk $? k_id); cases (pubk $? k_id); simplify_key_merges1; auto;
-          cases b; auto;
-            specialize (H _ _ Heq0); split_ands; subst; contra_map_lookup.
-
-      - cases (honestk $? k__sign); cases (pubk $? k__sign); simplify_key_merges1; auto;
-          cases b; auto;
-            specialize (H _ _ Heq0); split_ands; subst; contra_map_lookup.
+        cases v; unfold honest_keyb; simpl;
+          cases (honestk $? k__sign); cases (pubk $? k__sign); simplify_key_merges1; auto;
+            cases b; auto;
+              specialize (H _ _ Heq0); split_ands; subst; contra_map_lookup.
     Qed.
 
     Lemma clean_ciphers_nochange_pubk :
@@ -2776,25 +3154,23 @@ Section SingleAdversarySimulates.
     Qed.
 
     Lemma msg_filter_nochange_pubk :
-      forall honestk pubk m,
+      forall honestk pubk cs m,
         (forall k kp, pubk $? k = Some kp -> honestk $? k = Some true /\ kp = false)
-        -> msg_filter (honestk $k++ pubk) m = msg_filter honestk m.
+        -> msg_filter (honestk $k++ pubk) cs m = msg_filter honestk cs m.
     Proof.
-      unfold msg_filter, msg_honestly_signed; destruct m; intros; 
-        cases c; unfold honest_keyb; simpl; auto.
-      - cases (honestk $? k__sign); cases (pubk $? k__sign); simplify_key_merges1; auto;
-          destruct b; auto;
-            specialize (H _ _ Heq0); split_ands; subst; contra_map_lookup.
-
-      - cases (honestk $? k); cases (pubk $? k); simplify_key_merges1; auto;
-          destruct b; auto;
-            specialize (H _ _ Heq0); split_ands; subst; contra_map_lookup.
+      unfold msg_filter, msg_honestly_signed, msg_signing_key; destruct m; intros;
+        cases c; unfold honest_keyb; simpl; eauto;
+          cases (cs $? c_id); try discriminate; auto;
+            cases (honestk $? cipher_signing_key c); cases (pubk $? cipher_signing_key c);
+              simplify_key_merges1; eauto;
+                destruct b; eauto;
+                  specialize (H _ _ Heq1); split_ands; subst; contra_map_lookup.
     Qed.
 
     Lemma clean_messages_nochange_pubk :
-      forall honestk pubk qmsgs,
+      forall honestk pubk cs qmsgs,
         (forall k kp, pubk $? k = Some kp -> honestk $? k = Some true /\ kp = false)
-        -> clean_messages (honestk $k++ pubk) qmsgs = clean_messages honestk qmsgs.
+        -> clean_messages (honestk $k++ pubk) cs qmsgs = clean_messages honestk cs qmsgs.
     Proof.
       induction qmsgs; intros; eauto.
       simpl.
@@ -2859,9 +3235,9 @@ Section SingleAdversarySimulates.
     (* Qed. *)
 
     Lemma clean_users_nochange_pubk :
-      forall {A} (usrs: honest_users A) honestk pubk,
+      forall {A} (usrs: honest_users A) honestk cs pubk,
         (forall k kp, pubk $? k = Some kp -> honestk $? k = Some true /\ kp = false)
-        -> clean_users (honestk $k++ pubk) usrs = clean_users honestk usrs.
+        -> clean_users (honestk $k++ pubk) cs usrs = clean_users honestk cs usrs.
     Proof.
       intros; unfold clean_users.
       eapply map_eq_Equal; unfold Equal; intros.
@@ -2874,7 +3250,7 @@ Section SingleAdversarySimulates.
     Qed.
 
     Lemma clean_users_nochange_pubk_step :
-      forall {A} (usrs: honest_users A) honestk pubk u_id ks cmd qmsgs mycs u_d u_d',
+      forall {A} (usrs: honest_users A) honestk cs pubk u_id ks cmd qmsgs mycs u_d u_d',
         (forall k kp, pubk $? k = Some kp -> honestk $? k = Some true /\ kp = false)
         -> u_d = {| key_heap := ks $k++ pubk
                  ; protocol := cmd
@@ -2882,10 +3258,10 @@ Section SingleAdversarySimulates.
                  ; c_heap := mycs |}
         -> u_d' = {| key_heap := clean_key_permissions honestk (ks $k++ pubk)
                   ; protocol := cmd
-                  ; msg_heap := clean_messages honestk qmsgs
+                  ; msg_heap := clean_messages honestk cs qmsgs
                   ; c_heap := mycs |}
-        -> clean_users (honestk $k++ pubk) (usrs $+ (u_id,u_d)) =
-          clean_users honestk usrs $+ (u_id,u_d').
+        -> clean_users (honestk $k++ pubk) cs (usrs $+ (u_id,u_d)) =
+          clean_users honestk cs usrs $+ (u_id,u_d').
     Proof.
       intros.
       eapply map_eq_Equal; unfold Equal; intros.
@@ -2947,11 +3323,11 @@ Section SingleAdversarySimulates.
                 -> ud' = {| key_heap := ks'; protocol := cmdc'; msg_heap := qmsgs' ; c_heap := mycs' |}
                 -> usrs'' = usrs' $+ (u_id, ud')
                 -> clean_ciphers (findUserKeys usrs'') cs' = clean_ciphers (findUserKeys usrs') cs'
-                /\ clean_messages (findUserKeys usrs'') qmsgs' = clean_messages (findUserKeys usrs') qmsgs'
-                /\ clean_users (findUserKeys usrs'') usrs'' =
-                  clean_users (findUserKeys usrs') usrs' $+ (u_id, {| key_heap := clean_key_permissions (findUserKeys usrs') ks'
+                /\ clean_messages (findUserKeys usrs'') cs' qmsgs' = clean_messages (findUserKeys usrs') cs' qmsgs'
+                /\ clean_users (findUserKeys usrs'') cs' usrs'' =
+                  clean_users (findUserKeys usrs') cs' usrs' $+ (u_id, {| key_heap := clean_key_permissions (findUserKeys usrs') ks'
                                                                     ; protocol := cmdc'
-                                                                    ; msg_heap := clean_messages (findUserKeys usrs') qmsgs'
+                                                                    ; msg_heap := clean_messages (findUserKeys usrs') cs' qmsgs'
                                                                     ; c_heap := mycs' |})
                 /\ clean_adv adv' (findUserKeys usrs'') b = clean_adv adv' (findUserKeys usrs) b
                 /\ clean_keys (findUserKeys usrs'') gks' = clean_keys (findUserKeys usrs') gks'.
@@ -3024,6 +3400,24 @@ Section SingleAdversarySimulates.
       eapply honest_labeled_step_encrypted_ciphers_ok; eauto.
     Qed.
 
+    Lemma honest_message_findKeysCrypto_same_after_cleaning :
+      forall {t} (msg : crypto t) honestk cs,
+        msg_honestly_signed honestk cs msg = true
+        -> findKeysCrypto cs msg = findKeysCrypto (clean_ciphers honestk cs) msg.
+    Proof.
+      intros.
+      unfold message_no_adv_private, msg_honestly_signed, findKeysCrypto in *.
+      destruct msg; eauto.
+      cases (cs $? c_id); simpl in *; context_map_rewrites.
+      - destruct c; eauto;
+          eapply clean_ciphers_reduces_or_keeps_same_ciphers with (honestk := honestk) in Heq;
+          eauto; simpl in *; split_ors; split_ands; context_map_rewrites; eauto.
+        rewrite H in H1; discriminate.
+              
+      - eapply clean_ciphers_no_new_ciphers with (honestk := honestk) in Heq.
+        rewrite Heq; trivial.
+    Qed.
+
     Lemma honest_labeled_step_advuniv_implies_honest_step_origuniv :
       forall {A B C} cs cs' lbl u_id (usrs usrs' : honest_users A) (adv adv' : user_data B)
                 gks gks' ks ks' qmsgs qmsgs' mycs mycs' bd bd' a (b : B) suid,
@@ -3034,7 +3428,7 @@ Section SingleAdversarySimulates.
         -> forall (cmd : user_cmd C) cs__s usrs__s honestk,
           honestk = findUserKeys usrs
           -> cs__s = clean_ciphers honestk cs
-          -> usrs__s = clean_users honestk usrs
+          -> usrs__s = clean_users honestk cs usrs
           -> bd = (usrs, adv, cs, gks, ks, qmsgs, mycs, cmd)
           -> forall cmdc cmdc' usrs'' honestk',
               usrs $? u_id = Some {| key_heap := ks ; msg_heap := qmsgs ; protocol := cmdc ; c_heap := mycs |}
@@ -3042,7 +3436,7 @@ Section SingleAdversarySimulates.
               -> honestk' = findUserKeys usrs''
               -> forall cmd' cs__s' usrs__s' pwless_adv pwless_adv',
                   cs__s' = clean_ciphers honestk' cs'
-                  -> usrs__s' = clean_users honestk' usrs'
+                  -> usrs__s' = clean_users honestk' cs' usrs'
                   -> bd' = (usrs', adv', cs', gks', ks', qmsgs', mycs', cmd')
                   -> lbl = Action a
                   -> pwless_adv = {| key_heap := key_heap adv
@@ -3054,23 +3448,25 @@ Section SingleAdversarySimulates.
                                    ; msg_heap := adv'.(msg_heap)
                                    ; c_heap   := adv'.(c_heap) |}
                   -> step_user lbl suid
-                              (usrs__s, pwless_adv, cs__s, gks, ks, clean_messages honestk qmsgs, mycs, cmd)
-                              (usrs__s', pwless_adv', cs__s', gks', ks', clean_messages honestk' qmsgs', mycs', cmd').
+                              (usrs__s, pwless_adv, cs__s, gks, ks, clean_messages honestk cs qmsgs, mycs, cmd)
+                              (usrs__s', pwless_adv', cs__s', gks', ks', clean_messages honestk' cs' qmsgs', mycs', cmd').
     Proof.
       induction 1; inversion 7; inversion 6; intros;
         subst; try discriminate;
           try solve [ econstructor; eauto ];
           clean_context;
           autorewrite with find_user_keys.
-
  
-      - eapply Forall_natmap_in_prop in H8; eauto; invert H8.
-        split_ands. specialize_msg_ok.
+      - msg_queue_prop; split_ands; specialize_msg_ok.
         rewrite clean_users_nochange_pubk, clean_ciphers_nochange_pubk, clean_messages_nochange_pubk; eauto.
-        assert (msg_honestly_signed (findUserKeys usrs') msg = true) by eauto.
-            rewrite HON_SIGN; econstructor; eauto.
+        assert (msg_honestly_signed (findUserKeys usrs') cs' msg = true) as HON_SIGN by eauto.
+        rewrite HON_SIGN; econstructor; eauto.
+        erewrite honest_message_findKeysCrypto_same_after_cleaning; eauto.
 
-      - econstructor; eauto.
+      - econstructor;
+          try (erewrite <- honest_message_findKeysCrypto_same_after_cleaning by solve [ eauto ] );
+          eauto.
+        
         eapply clean_users_cleans_user; eauto.
         simpl.
         rewrite clean_users_add_pull; simpl.
@@ -3092,12 +3488,12 @@ Section SingleAdversarySimulates.
     Hint Resolve content_contains_only_honest_public_keys_keys_honest.
     
     Lemma message_contains_only_honest_public_keys_keys_honest :
-      forall {t} (msg : crypto t) k kp honestk,
-        msg_contains_only_honest_public_keys honestk msg
-        -> findKeysCrypto msg $? k = Some kp
+      forall {t} (msg : crypto t) k kp honestk cs,
+        msg_contains_only_honest_public_keys honestk cs msg
+        -> findKeysCrypto cs msg $? k = Some kp
         -> honestk $? k = Some true.
     Proof.
-      induction 1; simpl; intros; subst; clean_map_lookups; eauto.
+      induction 1; simpl; intros; subst; context_map_rewrites; clean_map_lookups; eauto.
     Qed.
 
     Lemma honest_labeled_step_advuniv_implies_honest_step_origuniv' :
@@ -3110,12 +3506,12 @@ Section SingleAdversarySimulates.
         -> forall (cmd : user_cmd C) cs__s usrs__s honestk,
           honestk = findUserKeys usrs
           -> cs__s = clean_ciphers honestk cs
-          -> usrs__s = clean_users honestk usrs
+          -> usrs__s = clean_users honestk cs usrs
           -> bd = (usrs, adv, cs, gks, ks, qmsgs, mycs, cmd)
           -> forall cmd' cs__s' usrs__s' honestk',
               honestk' = findUserKeys usrs'
               -> cs__s' = clean_ciphers honestk' cs'
-              -> usrs__s' = clean_users honestk' usrs'
+              -> usrs__s' = clean_users honestk' cs' usrs'
               -> bd' = (usrs', adv', cs', gks', ks', qmsgs', mycs', cmd')
               -> lbl = Action a
               -> user_queue usrs u_id = Some qmsgs
@@ -3124,9 +3520,9 @@ Section SingleAdversarySimulates.
                   -> a' = strip_action (findUserKeys usrs) a
                   -> step_user (Action a') suid
                               (usrs__s, clean_adv adv (findUserKeys usrs) b, cs__s, clean_keys honestk gks,
-                               clean_key_permissions honestk ks, clean_messages honestk qmsgs, mycs, cmd)
+                               clean_key_permissions honestk ks, clean_messages honestk cs qmsgs, mycs, cmd)
                               (usrs__s', clean_adv adv' (findUserKeys usrs) b, cs__s', clean_keys honestk' gks',
-                               clean_key_permissions honestk' ks', clean_messages honestk' qmsgs', mycs', cmd').
+                               clean_key_permissions honestk' ks', clean_messages honestk' cs' qmsgs', mycs', cmd').
     Proof.
       induction 1; inversion 7; inversion 4; intros;
         subst; try discriminate;
@@ -3134,23 +3530,26 @@ Section SingleAdversarySimulates.
           clean_context;
           autorewrite with find_user_keys.
 
-      - assert ( msg_honestly_signed (findUserKeys usrs') msg = true ) by eauto.
+      - assert ( msg_honestly_signed (findUserKeys usrs') cs' msg = true ) by eauto.
         rewrite H.
         econstructor; eauto.
 
-        msg_queue_prop.
+        msg_queue_prop. specialize_msg_ok.
+        erewrite <- honest_message_findKeysCrypto_same_after_cleaning by solve [ eauto ].
         rewrite clean_key_permissions_distributes_merge_key_permissions.
         
-        assert (clean_key_permissions (findUserKeys usrs') (findKeysCrypto msg) = findKeysCrypto msg).
+        assert (clean_key_permissions (findUserKeys usrs') (findKeysCrypto cs' msg) = findKeysCrypto cs' msg).
         + apply map_eq_Equal; unfold Equal; intros.
-          cases (findKeysCrypto msg $? y).
+          cases (findKeysCrypto cs' msg $? y).
           * apply clean_key_permissions_keeps_honest_permission; eauto.
-            specialize (H3 _ _ Heq); split_ands; subst; eauto.
+            specialize (H9 _ _ Heq); split_ands; subst; eauto.
           * apply clean_key_permissions_adds_no_permissions; eauto.
-        + rewrite H9; trivial.
+        + rewrite H12; trivial.
 
       - econstructor; eauto.
         + unfold keys_mine in *; intros.
+
+          erewrite <- honest_message_findKeysCrypto_same_after_cleaning in H6 by solve [ eauto ].
           pose proof (message_contains_only_honest_public_keys_keys_honest _ H H6).
           specialize (H0 _ _ H6); split_ors; split_ands; subst.
           * left; eapply clean_key_permissions_keeps_honest_permission; eauto.
@@ -3158,17 +3557,18 @@ Section SingleAdversarySimulates.
             eapply clean_key_permissions_keeps_honest_permission; eauto.
 
         + unfold clean_adv, addUserKeys; simpl.
-          destruct H; simpl in *; try discriminate; eauto.
+          erewrite <- honest_message_findKeysCrypto_same_after_cleaning by solve [ eauto ].
+          destruct H; simpl in *; try discriminate; context_map_rewrites; eauto.
           f_equal; eauto.
           rewrite clean_key_permissions_distributes_merge_key_permissions.
           apply map_eq_Equal; unfold Equal; intros.
-          cases (findKeysCrypto msg $? y).
-          * pose proof (message_contains_only_honest_public_keys_keys_honest _ H Heq).
-            assert (clean_key_permissions (findUserKeys usrs) (findKeysCrypto msg) $? y = Some b0).
+          cases (findKeysMessage m $? y).
+          * pose proof (content_contains_only_honest_public_keys_keys_honest _ H6 Heq).
+            assert (clean_key_permissions (findUserKeys usrs) (findKeysMessage m) $? y = Some b0).
             apply clean_key_permissions_keeps_honest_permission; eauto.
             unfold honest_perm_filter_fn; context_map_rewrites; trivial.
             cases (clean_key_permissions (findUserKeys usrs) (key_heap adv) $? y); simplify_key_merges; eauto.
-          * assert (clean_key_permissions (findUserKeys usrs) (findKeysCrypto msg) $? y = None).
+          * assert (clean_key_permissions (findUserKeys usrs) (findKeysMessage m) $? y = None).
             apply clean_key_permissions_adds_no_permissions; eauto.
             cases (clean_key_permissions (findUserKeys usrs) (key_heap adv) $? y); simplify_key_merges; eauto.
         + eapply clean_users_cleans_user; eauto.
@@ -3346,8 +3746,8 @@ Section SingleAdversarySimulates.
                 usrs $? u_id = Some {| key_heap := ks ; msg_heap := qmsgs ; protocol := cmdc ; c_heap := mycs |}
                 -> usrs'' = usrs' $+ (u_id, {| key_heap := ks'; protocol := cmdc'; msg_heap := qmsgs' ; c_heap := mycs' |})
                 ->  clean_ciphers (findUserKeys usrs'') cs' = clean_ciphers (findUserKeys usrs') cs'
-                /\ clean_messages (findUserKeys usrs'') qmsgs' = clean_messages (findUserKeys usrs') qmsgs'
-                /\ clean_users (findUserKeys usrs'') usrs' = clean_users (findUserKeys usrs') usrs'.
+                /\ clean_messages (findUserKeys usrs'') cs' qmsgs' = clean_messages (findUserKeys usrs') cs' qmsgs'
+                /\ clean_users (findUserKeys usrs'') cs' usrs' = clean_users (findUserKeys usrs') cs' usrs'.
     Proof.
       induction 1; inversion 2; inversion 6; intros; try discriminate; subst;
         autorewrite with find_user_keys; eauto; clean_context.
@@ -3406,12 +3806,13 @@ Section SingleAdversarySimulates.
         inversion H10; subst.
         unfold clean_adv; simpl; f_equal.
         + rewrite clean_users_add_pull; simpl.
-          assert (clean_users (findUserKeys users) users =
-                  clean_users (findUserKeys (usrs $+ (u_id, {| key_heap := ks; protocol := cmd; msg_heap := qmsgs; c_heap := mycs |}))) usrs).
+          assert (clean_users (findUserKeys users) all_ciphers users =
+                  clean_users (findUserKeys (usrs $+ (u_id, {| key_heap := ks; protocol := cmd; msg_heap := qmsgs; c_heap := mycs |}))) cs usrs).
           unfold clean_users, map; apply map_eq_elements_eq; simpl; auto.
           rewrite <- H11.
           apply map_eq_Equal; unfold Equal; intros.
-          destruct (y ==n u_id); subst; clean_map_lookups; trivial; eapply clean_users_cleans_user; eauto.
+          destruct (y ==n u_id); subst; clean_map_lookups; eauto.
+          eapply clean_users_cleans_user; eauto.
           f_equal; eauto.
         + f_equal; eauto.
 
@@ -3428,12 +3829,12 @@ Section SingleAdversarySimulates.
         -> forall (cmd : user_cmd C) honestk,
             honestk = findUserKeys usrs
             -> bd = (usrs, adv, cs, gks, ks, qmsgs, mycs, cmd)
-            -> usrs = clean_users honestk usrs__ra
+            -> usrs = clean_users honestk cs usrs__ra
             -> adv = clean_adv adv__ra honestk b
             -> cs = clean_ciphers honestk cs__ra
             -> gks = clean_keys honestk gks__ra
             -> ks = clean_key_permissions honestk ks__ra
-            -> qmsgs = clean_messages honestk qmsgs__ra
+            -> qmsgs = clean_messages honestk cs qmsgs__ra
             -> forall cmd' bd__ra' a__ra,
                 bd' = (usrs', adv', cs', gks', ks', qmsgs', mycs', cmd')
                 -> bd__ra' = (usrs__ra', adv__ra', cs__ra', gks__ra', ks__ra', qmsgs__ra', mycs', cmd')
@@ -3484,11 +3885,11 @@ Section SingleAdversarySimulates.
         remember (x2 $+ (x, {| key_heap := x6; protocol := x9; msg_heap := x7 ; c_heap := x8 |})) as usrs''.
 
         assert (clean_ciphers (findUserKeys usrs'') x4 = clean_ciphers (findUserKeys x2) x4
-              /\ clean_messages (findUserKeys usrs'') x7 = clean_messages (findUserKeys x2) x7
-              /\ clean_users (findUserKeys usrs'') usrs'' =
-                clean_users (findUserKeys x2) x2 $+ (x, {| key_heap := clean_key_permissions (findUserKeys x2) x6
+              /\ clean_messages (findUserKeys usrs'') x4 x7 = clean_messages (findUserKeys x2) x4 x7
+              /\ clean_users (findUserKeys usrs'') x4 usrs'' =
+                clean_users (findUserKeys x2) x4 x2 $+ (x, {| key_heap := clean_key_permissions (findUserKeys x2) x6
                                                          ; protocol := x9
-                                                         ; msg_heap := clean_messages (findUserKeys x2) x7
+                                                         ; msg_heap := clean_messages (findUserKeys x2) x4 x7
                                                          ; c_heap := x8 |})
               /\ clean_adv x3 (findUserKeys usrs'') b = clean_adv x3 (findUserKeys users) b
               /\ clean_keys (findUserKeys usrs'') x5 = clean_keys (findUserKeys x2) x5 ).
@@ -3595,11 +3996,11 @@ Section SingleAdversarySimulates.
             bd = (usrs, adv, cs, gks, adv.(key_heap), adv.(msg_heap), adv.(c_heap), cmd)
           -> honestk = findUserKeys usrs
           -> adv_no_honest_keys (findUserKeys usrs) adv.(key_heap)
-          -> usrs__s = clean_users honestk usrs
+          -> usrs__s = clean_users honestk cs usrs
           -> forall cmd' honestk' usrs__s',
                 bd' = (usrs', adv', cs', gks', ks', qmsgs', mycs', cmd')
               -> honestk' = findUserKeys usrs'
-              -> usrs__s' = clean_users honestk' usrs'
+              -> usrs__s' = clean_users honestk' cs' usrs'
               -> usrs__s = usrs__s'.
     Proof.
       induction 1; inversion 1; inversion 4; intros; subst; eauto.
@@ -3613,7 +4014,7 @@ Section SingleAdversarySimulates.
       clear H6 H18.
 
       erewrite clean_users_cleans_user; eauto; f_equal.
-      cases (msg_honestly_signed (findUserKeys usrs) msg);
+      cases (msg_honestly_signed (findUserKeys usrs) cs' msg);
         eauto using clean_messages_drops_not_honestly_signed.
 
       exfalso.
@@ -3660,6 +4061,44 @@ Section SingleAdversarySimulates.
         trivial.
     Qed.
 
+    Lemma encrypted_ciphers_ok_new_honest_cipher_adv_univ :
+      forall honestk cs cs' c_id c k gks,
+        ~ In c_id cs
+        -> cs' = cs $+ (c_id,c)
+        -> cipher_signing_key c = k
+        -> honest_key honestk k
+        -> encrypted_ciphers_ok honestk cs gks
+        -> encrypted_ciphers_ok honestk (clean_ciphers honestk cs') gks
+        -> encrypted_ciphers_ok honestk cs' gks.
+    Proof.
+      intros; subst.
+      rewrite clean_ciphers_keeps_added_honest_cipher in H4; simpl; eauto.
+      eapply Forall_natmap_split in H4; split_ands; eauto.
+      econstructor; eauto.
+      invert H1; solve [ econstructor; eauto ].
+    Qed.
+
+    Hint Resolve encrypted_ciphers_ok_new_honest_cipher_adv_univ.
+
+    Lemma encrypted_ciphers_ok_new_honest_key_adv_univ :
+      forall honestk honestk' cs k_id k gks gks',
+        ~ In k_id gks
+        -> permission_heap_good gks honestk
+        -> k_id = keyId k
+        -> gks' = gks $+ (k_id, k)
+        -> honestk' = honestk $+ (k_id, true)
+        -> encrypted_ciphers_ok honestk cs gks
+        -> encrypted_ciphers_ok honestk' (clean_ciphers honestk' cs) gks'
+        -> encrypted_ciphers_ok honestk' cs gks'.
+    Proof.
+      intros; subst; eapply encrypted_ciphers_ok_addnl_honest_key; eauto.
+      cases (honestk $? keyId k); clean_map_lookups; eauto.
+      specialize (H0 _ _ Heq); split_ex; contra_map_lookup.
+    Qed.
+
+    Hint Resolve encrypted_ciphers_ok_new_honest_key_adv_univ.
+    Hint Resolve users_permission_heaps_good_merged_permission_heaps_good.
+
     Lemma honest_silent_step_adv_univ_enc_ciphers_ok' :
       forall {A B C} cs cs' u_id suid lbl (usrs usrs' : honest_users A) (adv adv' : user_data B)
                 gks gks' ks ks' qmsgs qmsgs' mycs mycs' bd bd',
@@ -3684,69 +4123,15 @@ Section SingleAdversarySimulates.
         try discriminate;
         eauto 2;
         autorewrite with find_user_keys in *;
-        eauto.
-
-      - rewrite clean_ciphers_keeps_added_honest_cipher in H35; simpl; eauto.
-        eapply Forall_natmap_split in H35; auto; split_ands.
-        econstructor; eauto.
-        + assert ( (findUserKeys usrs') $? k__signid = Some true) by eauto.
-          invert H7; try contradiction.
-          eapply SigEncCipherHonestSignedEncKeyHonestOk; eauto.
-          unfold msgCiphersSignedOk in *.
-          rewrite Forall_forall in *; intros.
-          specialize (H25 _ H7).
-          unfold msgCipherOk in *; destruct x; intuition idtac.
-          destruct c; eauto.
-          * split_ex.
-            repeat eexists.
-            cases (c_id ==n msg_id); subst; clean_map_lookups; eauto.
-            rewrite <- find_mapsto_iff in H9; rewrite clean_ciphers_mapsto_iff in H9; split_ands; auto.
-            rewrite find_mapsto_iff in H9; auto.
-          * cases (c_id ==n sig); subst; clean_map_lookups; eauto.
-            rewrite <- find_mapsto_iff in H9; rewrite clean_ciphers_mapsto_iff in H9; split_ands; auto.
-            rewrite find_mapsto_iff in H9; auto.
-        + apply encrypted_ciphers_ok_addnl_cipher; auto.
+        keys_and_permissions_prop;
+        eauto;
+        clean_context.
 
       - user_cipher_queues_prop.
         encrypted_ciphers_prop.
         rewrite merge_keys_addnl_honest; eauto.
-
-      - rewrite clean_ciphers_keeps_added_honest_cipher in H31; simpl; eauto.
-        eapply Forall_natmap_split in H31; auto; split_ands.
-        assert (findUserKeys usrs' $? k_id = Some true) by eauto.
-        invert H3; try contradiction.
-        econstructor; eauto.
-        + econstructor; eauto.
-          unfold msgCiphersSignedOk in *.
-          rewrite Forall_forall in *; intros.
-          specialize (H14 _ H3).
-          unfold msgCipherOk in *; destruct x; intuition idtac.
-          destruct c; eauto.
-          * split_ex.
-            repeat eexists.
-            cases (c_id ==n msg_id); subst; clean_map_lookups; eauto.
-            rewrite <- find_mapsto_iff in H5; rewrite clean_ciphers_mapsto_iff in H5; split_ands; auto.
-            rewrite find_mapsto_iff in H5; eauto.
-          * cases (c_id ==n sig); subst; clean_map_lookups; eauto.
-            rewrite <- find_mapsto_iff in H5; rewrite clean_ciphers_mapsto_iff in H5; split_ands; auto.
-            rewrite find_mapsto_iff in H5; auto.
-        + eapply encrypted_ciphers_ok_addnl_cipher; auto.
-
-      - clean_context.
-        assert (permission_heap_good gks (findUserKeys usrs'))
-          by (unfold keys_and_permissions_good in *; split_ands; eauto using users_permission_heaps_good_merged_permission_heaps_good).
-        eapply encrypted_ciphers_ok_addnl_honest_key; simpl; eauto.
-        unfold permission_heap_good in *.
-        cases (findUserKeys usrs' $? k_id); clean_map_lookups; eauto.
-        specialize (H0 _ _ Heq); split_ex; contra_map_lookup.
-
-      - clean_context.
-        assert (permission_heap_good gks (findUserKeys usrs'))
-          by (unfold keys_and_permissions_good in *; split_ands; eauto using users_permission_heaps_good_merged_permission_heaps_good).
-        eapply encrypted_ciphers_ok_addnl_honest_key; simpl; eauto.
-        unfold permission_heap_good in *.
-        cases (findUserKeys usrs' $? k_id); clean_map_lookups; eauto.
-        specialize (H0 _ _ Heq); split_ex; contra_map_lookup.
+      - eapply encrypted_ciphers_ok_new_honest_key_adv_univ with (honestk := (findUserKeys usrs')); simpl; eauto; simpl; eauto.
+      - eapply encrypted_ciphers_ok_new_honest_key_adv_univ with (honestk := (findUserKeys usrs')); simpl; eauto; simpl; eauto.
     Qed.
 
     Lemma clean_ciphers_eq_absurd :
@@ -3808,12 +4193,12 @@ Section SingleAdversarySimulates.
         autorewrite with find_user_keys in *;
         eauto; clean_context.
 
-      - exfalso; invert H37.
-        erewrite clean_ciphers_added_honest_cipher_not_cleaned in H9; eauto.
+      - exfalso; invert H36.
+        erewrite clean_ciphers_added_honest_cipher_not_cleaned in H8; eauto.
         2: simpl; econstructor; rewrite findUserKeys_readd_user_same_keys_idempotent'; eauto.
-        rewrite !findUserKeys_readd_user_same_keys_idempotent' in H9; eauto.
+        rewrite !findUserKeys_readd_user_same_keys_idempotent' in H8; eauto.
 
-      - invert H37.
+      - invert H36.
         user_cipher_queues_prop.
         encrypted_ciphers_prop.
         rewrite merge_keys_addnl_honest; eauto.
@@ -3926,7 +4311,7 @@ Section SingleAdversarySimulates.
         destruct U__ra; destruct U__ra'; simpl in *.
         unfold strip_adversary_univ in *; unfold strip_adversary in *; simpl in *.
         invert H4; auto.
-        assert (clean_users (RealWorld.findUserKeys users) users = clean_users (RealWorld.findUserKeys users0) users0)
+        assert (clean_users (RealWorld.findUserKeys users) all_ciphers users = clean_users (RealWorld.findUserKeys users0) all_ciphers0 users0)
           as CLEAN_USERS by (unfold clean_users, map; auto).
         rewrite <- CLEAN_USERS; auto.
 
@@ -4006,16 +4391,16 @@ Section SingleAdversarySimulates.
 
   Definition universe_starts_ok {A B} (U : RealWorld.universe A B) :=
     let honestk := RealWorld.findUserKeys U.(RealWorld.users)
-    in Forall_natmap (fun u => Forall (fun m => msg_filter honestk m = true) u.(RealWorld.msg_heap)
+    in Forall_natmap (fun u => Forall (fun m => msg_filter honestk U.(RealWorld.all_ciphers) m = true) u.(RealWorld.msg_heap)
                           /\ (forall k_id kp, u.(RealWorld.key_heap) $? k_id = Some kp -> honestk $? k_id = Some true)) U.(RealWorld.users)
       /\ Forall_natmap (fun c => RealWorld.cipher_honestly_signed honestk c = true) U.(RealWorld.all_ciphers)
       /\ Forall_natmap (fun k => RealWorld.honest_key honestk k.(keyId)) U.(RealWorld.all_keys)
   .
 
   Lemma clean_honest_messages_idempotent :
-    forall msgs honestk,
-      Forall (fun m => msg_filter honestk m = true) msgs
-      -> clean_messages honestk msgs = msgs.
+    forall cs msgs honestk,
+      Forall (fun m => msg_filter honestk cs m = true) msgs
+      -> clean_messages honestk cs msgs = msgs.
   Proof.
     induction msgs; eauto; intros.
     invert H.
@@ -4072,11 +4457,11 @@ Section SingleAdversarySimulates.
   Qed.
 
   Lemma universe_starts_ok_clean_users_idempotent :
-    forall {A} (usrs : RealWorld.honest_users A) honestk,
+    forall {A} (usrs : RealWorld.honest_users A) honestk cs,
       honestk = RealWorld.findUserKeys usrs
-      -> Forall_natmap (fun u => Forall (fun m => msg_filter honestk m = true) u.(RealWorld.msg_heap)
+      -> Forall_natmap (fun u => Forall (fun m => msg_filter honestk cs m = true) u.(RealWorld.msg_heap)
                            /\ (forall k_id kp, u.(RealWorld.key_heap) $? k_id = Some kp -> honestk $? k_id = Some true)) usrs
-      -> clean_users honestk usrs = usrs.
+      -> clean_users honestk cs usrs = usrs.
   Proof.
     intros.
     rewrite Forall_natmap_forall in *.
